pilot/shared/M2_REDEX_ORACLE.sexp
@@ -1,0 +1,2690 @@
+(smusni-m2-redex-oracle
+ 1
+ (count 160)
+ (cases
+  (case (id "0347d6a60531d233b4926705a0d467d921d7f383")
+    (status available)
+    (term
+     (Ask
+      (Polar
+       (Bind
+        ($ctx2 :: (Referents Entity))
+        (Context)
+        ($ctx3 :: (Referents Entity))
+        (Context)
+        ($ctx4 :: (Referents Entity))
+        (Context)
+        ($ctx5 :: (Referents Entity))
+        (Context)
+        (CloseClause
+         (λ (($actual_event :: (Referents Eventuality)))
+           (∧
+            ((λ (($event :: (Referents Eventuality))) (klama Speaker $ctx2 $ctx3 $ctx4 $ctx5 $event)) $actual_event)
+            (fasnu $actual_event)))))))))
+  (case (id "04cdfd2f45e14a4ad9d525b9aa39518337dfe160")
+    (status available)
+    (term
+     (∧
+      ((λ (($left :: (Referents Entity)) ($right :: (Referents Entity)))
+         (Bind
+          ($ctx3 :: (Referents Entity))
+          (Context)
+          (CloseClause
+           (λ (($actual_event :: (Referents Eventuality)))
+             (∧
+              ((λ (($event :: (Referents Eventuality))) (tavla $left $right $ctx3 $event)) $actual_event)
+              (fasnu $actual_event))))))
+       Speaker
+       Audience)
+      (∧
+       ((λ (($left :: (Referents Entity)) ($right :: (Referents Entity)))
+          (Bind
+           ($ctx3 :: (Referents Entity))
+           (Context)
+           (CloseClause
+            (λ (($actual_event :: (Referents Eventuality)))
+              (∧
+               ((λ (($event :: (Referents Eventuality))) (tavla $left $right $ctx3 $event)) $actual_event)
+               (fasnu $actual_event))))))
+        Audience
+        Speaker)
+       (∧)))))
+  (case (id "08b939906bc81531981e2e136544295588e28456")
+    (status available)
+    (term
+     (Bind
+      ($w :: (Referents Entity))
+      (SelectExactly 3 (λ (($x :: Entity)) (gerku $x)))
+      (Mention
+       (Bind
+        ($ctx2 :: (Referents Entity))
+        (Context)
+        ($ctx3 :: (Referents Entity))
+        (Context)
+        ($ctx4 :: (Referents Entity))
+        (Context)
+        (CloseClause
+         (λ (($actual_event :: (Referents Eventuality)))
+           (∧
+            ((λ (($event :: (Referents Eventuality))) (bajra $w $ctx2 $ctx3 $ctx4 $event)) $actual_event)
+            (fasnu $actual_event)))))))))
+  (case (id "08f992b5f049f24666cf4ace53d35d90dea91c37")
+    (status available)
+    (term
+     (SentenceSign
+      (Bind
+       ($x :: Entity)
+       (Context)
+       (Bind
+        ($ctx2 :: (Referents Entity))
+        (Context)
+        ($ctx3 :: (Referents Entity))
+        (Context)
+        ($ctx4 :: (Referents Entity))
+        (Context)
+        ($ctx5 :: (Referents Entity))
+        (Context)
+        (CloseClause
+         (λ (($actual_event :: (Referents Eventuality)))
+           (∧
+            ((λ (($event :: (Referents Eventuality))) (klama $x $ctx2 $ctx3 $ctx4 $ctx5 $event)) $actual_event)
+            (fasnu $actual_event)))))))))
+  (case (id "0aca32fd93634be168dabf02d8e7156122b58fc3")
+    (status unavailable)
+    (reason
+     "b1-expand-no: (b1-expand-no Entity (λ (($x Entity)) (Bind (($s Scale (Context))) (gerku $x))) (λ (($w (Referents Entity))) (CloseWith (row jmaji 1 direct-event (1)) ((1 $w))))) is not in my domain"))
+  (case (id "0b9143a8dcab3aa4be92bcca72f9cfccf0bf8651")
+    (status available)
+    (term
+     (Assert
+      (Bind
+       ($w1 :: (Referents Entity))
+       (Presuppose
+        (∃ (λ (($x :: Entity)) (gerku $x)))
+        (Refer
+         (λ (($reference :: (Referents Entity)))
+           (∧
+            (∧
+             (∀ (λ (($member :: Entity)) (→ (Among $member $reference) ((λ (($x :: Entity)) (gerku $x)) $member))))
+             (∀
+              (λ (($subreference :: (Referents Entity)))
+                (→
+                 (Among $subreference $reference)
+                 (∃
+                  (λ (($member :: Entity))
+                    (∧
+                     ((λ (($x :: Entity)) (gerku $x)) $member)
+                     (∃
+                      (λ (($common :: (Referents Entity)))
+                        (∧ (Among $common $member) (Among $common $subreference)))))))))))
+            (∀ (λ (($member :: Entity)) (→ ((λ (($x :: Entity)) (gerku $x)) $member) (Among $member $reference))))))))
+       (∀
+        (λ (($member :: Entity))
+          (→
+           (Among $member $w1)
+           ((λ (($x :: Entity))
+              (Bind
+               ($w1 :: (Referents Entity))
+               (SelectAtLeast 1 (λ (($x :: Entity)) (mlatu $x)))
+               ((λ (($w :: (Referents Entity)))
+                  (Bind
+                   ($ctx3 :: (Referents Entity))
+                   (Context)
+                   (CloseClause
+                    (λ (($actual_event :: (Referents Eventuality)))
+                      (∧
+                       ((λ (($event :: (Referents Eventuality))) (tavla $x $w $ctx3 $event)) $actual_event)
+                       (fasnu $actual_event))))))
+                $w1)))
+            $member))))))))
+  (case (id "0c9cfd6de375ffa1d4fff442d727306600ec85f1")
+    (status unavailable)
+    (reason
+     "a0-expand-let: (a0-expand-let $a (Act Assertion) (Assert (CloseWith (row klama 5 direct-event (1 2 3 4 5)) ((1 Speaker)))) (Bind (($o (ActOccurrence Assertion) (Perform Host $a))) (Do (Perform AttachedDisplay (Express (Close (Happiness Speaker $o Moderate))))))) is not in my domain"))
+  (case (id "0dc79107606886122b69471a7a186d8eac5a1230")
+    (status available)
+    (term
+     (Bind
+      ($left :: (Referents Entity))
+      (SelectExactly 3 (λ (($x :: Entity)) (gerku $x)))
+      ($right :: (Referents Entity))
+      (SelectExactly 2 (λ (($x1 :: Entity)) (prenu $x1)))
+      (Assert
+       (∀
+        (λ (($member :: Entity))
+          (→
+           (Among $member $left)
+           ((λ (($l :: Entity))
+              (∀
+               (λ (($member :: Entity))
+                 (→
+                  (Among $member $right)
+                  ((λ (($r :: Entity))
+                     (CloseClause
+                      (λ (($actual_event :: (Referents Eventuality)))
+                        (∧ ((StateClause (nelci $l $r)) $actual_event) (fasnu $actual_event)))))
+                   $member)))))
+            $member))))))))
+  (case (id "1089e66a065f6aff2907dbf77e625afb9dabf755")
+    (status available)
+    (term
+     (Bind
+      ($alis :: (Referents Entity))
+      (Refer (λ (($x :: (Referents Entity))) (Named "alis" $x)))
+      (Assert
+       (Bind
+        ($ctx2 :: (Referents Entity))
+        (Context)
+        ($ctx3 :: (Referents Entity))
+        (Context)
+        ($ctx4 :: (Referents Entity))
+        (Context)
+        ($ctx5 :: (Referents Entity))
+        (Context)
+        (CloseClause
+         (λ (($actual_event :: (Referents Eventuality)))
+           (∧
+            ((λ (($event :: (Referents Eventuality))) (klama $alis $ctx2 $ctx3 $ctx4 $ctx5 $event)) $actual_event)
+            (fasnu $actual_event)))))))))
+  (case (id "10f71e5c385cb2118c01d8439fe7d8991a7db15a")
+    (status available)
+    (term
+     (Bind
+      ($scale :: (Referents Scale))
+      (Context)
+      (Bind
+       ($amt :: (Referents Amount))
+       (Refer
+        (λ (($a :: (Referents Amount)))
+          ((NiRel
+            (Bind
+             ($ctx2 :: (Referents Entity))
+             (Context)
+             ($ctx3 :: (Referents Entity))
+             (Context)
+             ($ctx4 :: (Referents Entity))
+             (Context)
+             ($ctx5 :: (Referents Entity))
+             (Context)
+             (CloseClause
+              (λ (($actual_event :: (Referents Eventuality)))
+                (∧
+                 ((λ (($event :: (Referents Eventuality))) (klama Speaker $ctx2 $ctx3 $ctx4 $ctx5 $event))
+                  $actual_event)
+                 (fasnu $actual_event))))))
+           $a
+           $scale)))
+       (Mention (− 1 (AmountValue $amt $scale)))))))
+  (case (id "1341fba432fc31883c7f2d4446847faa032bdea4")
+    (status unavailable)
+    (reason
+     "b1-expand-at-least: (b1-expand-at-least 1 Entity (λ (($x Entity)) (gerku $x)) (λ (($w (Referents Entity))) (Bind (($s Scale (Context))) (CloseWith (row jmaji 1 direct-event (1)) ((1 $w)))))) is not in my domain"))
+  (case (id "1b5d8a8c9fc9f9c06284e64734fc8ff9e530d6f9")
+    (status available)
+    (term (Bind ($w :: (Referents Entity)) (SelectAtLeast 1 (λ (($x :: Entity)) (gerku $x))) (Mention $w))))
+  (case (id "1daf460b64ca380a9652b69a2b4870ff4d842e2a")
+    (status unavailable)
+    (reason
+     "b1-expand-some: (b1-expand-some Entity (λ (($x Entity)) (Bind (($s Scale (Context))) (gerku $x))) (λ (($w (Referents Entity))) (CloseWith (row jmaji 1 direct-event (1)) ((1 $w))))) is not in my domain"))
+  (case (id "1f879cecd53e2fce98547b4d8ef87f2446308ebe")
+    (status available)
+    (term
+     (Bind
+      ($nuclear_klama_2 :: (Referents Entity))
+      (Context)
+      ($nuclear_klama_3 :: (Referents Entity))
+      (Context)
+      ($nuclear_klama_4 :: (Referents Entity))
+      (Context)
+      ($nuclear_klama_5 :: (Referents Entity))
+      (Context)
+      (=
+       (Card
+        (SetOf
+         (λ (($global_member :: Entity))
+           (∧
+            ((λ (($restrictor_member :: Entity)) (prenu $restrictor_member)) $global_member)
+            ((λ (($nuclear_member :: Entity))
+               (CloseClause
+                (λ (($actual_event :: (Referents Eventuality)))
+                  (∧
+                   ((λ (($event :: (Referents Eventuality)))
+                      (klama
+                       $nuclear_member
+                       $nuclear_klama_2
+                       $nuclear_klama_3
+                       $nuclear_klama_4
+                       $nuclear_klama_5
+                       $event))
+                    $actual_event)
+                   (fasnu $actual_event)))))
+             $global_member)))))
+       2))))
+  (case (id "24a8f6ee7b1b963841362803c17af2271ae6a6d9")
+    (status available)
+    (term
+     (SetOf
+      (λ (($z :: Entity))
+        (Bind
+         ($w1 :: (Referents Entity))
+         (SelectAtLeast 1 (λ (($x :: Entity)) (gerku $x)))
+         ((λ (($w :: (Referents Entity)))
+            (CloseClause
+             (λ (($actual_event :: (Referents Eventuality)))
+               (∧ ((λ (($event :: (Referents Eventuality))) (jmaji $w $event)) $actual_event) (fasnu $actual_event)))))
+          $w1))))))
+  (case (id "25087496e92097ae61f36b808ff5f741839aa26b")
+    (status available)
+    (term
+     (Bind
+      ($r :: (PredTerm (Row (1 (Referents Entity)) (2 (Referents Entity)))))
+      (Context)
+      (Assert (Close ($r Speaker Audience))))))
+  (case (id "258b2f3c9ce1b2f40ce28b1d99b981a3b7eed627")
+    (status unavailable)
+    (reason
+     "a0-expand-global-exactly: (a0-expand-global-exactly 1 Entity (λ (($x Entity)) (gerku $x)) (λ (($x Entity)) (Bind (($s Scale (Context))) (CloseWith (row jmaji 1 direct-event (1)) ((1 $x)))))) is not in my domain"))
+  (case (id "274806f8603d12078502192f6527633e6c13994d")
+    (status available)
+    (term
+     (Bind
+      ($r :: (Referents Entity))
+      (SelectExactly 3 (λ (($x :: Entity)) (gerku $x)))
+      (Assert
+       (Bind
+        ($ctx3 :: (Referents Entity))
+        (Context)
+        (CloseClause
+         (λ (($actual_event :: (Referents Eventuality)))
+           (∧
+            ((λ (($event :: (Referents Eventuality))) (tavla Speaker $r $ctx3 $event)) $actual_event)
+            (fasnu $actual_event)))))))))
+  (case (id "27f27c1038df83b40e16a919fdaf24b405d04b04")
+    (status available)
+    (term
+     (SetOf
+      (λ (($z :: Entity))
+        (Bind
+         ($w1 :: (Referents Entity))
+         (SelectAtLeast (+ 0 1) (λ (($x :: Entity)) (gerku $x)))
+         ((λ (($w :: (Referents Entity)))
+            (CloseClause
+             (λ (($actual_event :: (Referents Eventuality)))
+               (∧ ((λ (($event :: (Referents Eventuality))) (jmaji $w $event)) $actual_event) (fasnu $actual_event)))))
+          $w1))))))
+  (case (id "29cc86f6cefefcc0e82f7cc9606345c99e91b446")
+    (status unavailable)
+    (reason
+     "b1-expand-at-least: no clauses matched for (b1-expand-at-least $n Entity (λ (($x Entity)) (prenu $x)) (λ (($w (Referents Entity))) (CloseWith (row klama 5 direct-event (1 2 3 4 5)) ((1 $w)))))"))
+  (case (id "2a7470be1e19c3e1181aa00354f7d2f741d424e0")
+    (status available)
+    (term
+     (Bind
+      ($w1 :: (Referents Entity))
+      (SelectAtLeast 1 (λ (($x :: Entity)) (gerku $x)))
+      ((λ (($w :: (Referents Entity)))
+         (CloseClause
+          (λ (($actual_event :: (Referents Eventuality)))
+            (∧ ((λ (($event :: (Referents Eventuality))) (jmaji $w $event)) $actual_event) (fasnu $actual_event)))))
+       $w1))))
+  (case (id "2aef1b5ba045c6dddd31e5b6c700ea6ba5769506")
+    (status unavailable)
+    (reason
+     "b1-expand-at-most: (b1-expand-at-most 1 Entity (λ (($x Entity)) (gerku $x)) (λ (($w (Referents Entity))) (Bind (($s Scale (Context))) (CloseWith (row jmaji 1 direct-event (1)) ((1 $w)))))) is not in my domain"))
+  (case (id "2b5c18cc087f6f317b301f14f4f395bfc2ca10bd")
+    (status available)
+    (term
+     (Bind
+      ($restrictor_klama_2 :: (Referents Entity))
+      (Context)
+      ($restrictor_klama_3 :: (Referents Entity))
+      (Context)
+      ($restrictor_klama_4 :: (Referents Entity))
+      (Context)
+      ($restrictor_klama_5 :: (Referents Entity))
+      (Context)
+      ($nuclear_tavla_3 :: (Referents Entity))
+      (Context)
+      (Assert
+       (=
+        (Card
+         (SetOf
+          (λ (($global_member :: Entity))
+            (∧
+             ((λ (($restrictor_member :: Entity))
+                (CloseClause
+                 (λ (($actual_event :: (Referents Eventuality)))
+                   (∧
+                    ((λ (($event :: (Referents Eventuality)))
+                       (klama
+                        $restrictor_member
+                        $restrictor_klama_2
+                        $restrictor_klama_3
+                        $restrictor_klama_4
+                        $restrictor_klama_5
+                        $event))
+                     $actual_event)
+                    (fasnu $actual_event)))))
+              $global_member)
+             ((λ (($nuclear_member :: Entity))
+                (CloseClause
+                 (λ (($actual_event :: (Referents Eventuality)))
+                   (∧
+                    ((λ (($event :: (Referents Eventuality))) (tavla $nuclear_member Speaker $nuclear_tavla_3 $event))
+                     $actual_event)
+                    (fasnu $actual_event)))))
+              $global_member)))))
+        3)))))
+  (case (id "2bbd7ecacd72e5bf39fddcbd8685bbb0c8a298e1")
+    (status available)
+    (term
+     (Bind
+      ($r :: (Referents Entity))
+      (Refer (λ (($unit :: (Referents Entity))) (gerku $unit)))
+      (Assert
+       (Bind
+        ($ctx3 :: (Referents Entity))
+        (Context)
+        (CloseClause
+         (λ (($actual_event :: (Referents Eventuality)))
+           (∧
+            ((λ (($event :: (Referents Eventuality))) (tavla Speaker $r $ctx3 $event)) $actual_event)
+            (fasnu $actual_event)))))))))
+  (case (id "2dfd6a966b56f57fcae90ce8b9fc26926509c8cb")
+    (status available)
+    (term
+     (Bind
+      ($r :: (Referents Entity))
+      (Refer (λ (($unit :: (Referents Entity))) (gerku $unit)))
+      (Bind
+       ($r1 :: (Referents Entity))
+       (Refer (λ (($named :: (Referents Entity))) (Named "alis" $named)))
+       (Assert
+        (Bind
+         ($ctx3 :: (Referents Entity))
+         (Context)
+         (CloseClause
+          (λ (($actual_event :: (Referents Eventuality)))
+            (∧
+             ((λ (($event :: (Referents Eventuality))) (tavla $r $r1 $ctx3 $event)) $actual_event)
+             (fasnu $actual_event))))))))))
+  (case (id "2fcf22efb7f6212bf8ca744449fafda776c6f1c5")
+    (status available)
+    (term
+     (Assert
+      (¬
+       (Bind
+        ($w1 :: (Referents Entity))
+        (SelectAtLeast 1 (λ (($x :: Entity)) (mlatu $x)))
+        ((λ (($w :: (Referents Entity)))
+           (CloseClause
+            (λ (($actual_event :: (Referents Eventuality)))
+              (∧ ((StateClause (blabi $w)) $actual_event) (fasnu $actual_event)))))
+         $w1))))))
+  (case (id "302aef64343959ab2259e4b2226ebbda2a9f188c")
+    (status available)
+    (term
+     (Bind
+      ($cats :: (Referents Entity))
+      (Refer (λ (($x :: (Referents Entity))) (mlatu $x)))
+      (Assert
+       (Bind
+        ($w :: (Referents Entity))
+        (Presuppose
+         (∃ (λ (($x :: Entity)) (gerku $x)))
+         (Refer
+          (λ (($reference :: (Referents Entity)))
+            (∧
+             (∧
+              (∀ (λ (($member :: Entity)) (→ (Among $member $reference) ((λ (($x :: Entity)) (gerku $x)) $member))))
+              (∀
+               (λ (($subreference :: (Referents Entity)))
+                 (→
+                  (Among $subreference $reference)
+                  (∃
+                   (λ (($member :: Entity))
+                     (∧
+                      ((λ (($x :: Entity)) (gerku $x)) $member)
+                      (∃
+                       (λ (($common :: (Referents Entity)))
+                         (∧ (Among $common $member) (Among $common $subreference)))))))))))
+             (∀ (λ (($member :: Entity)) (→ ((λ (($x :: Entity)) (gerku $x)) $member) (Among $member $reference))))))))
+        (∀
+         (λ (($member :: Entity))
+           (→
+            (Among $member $w)
+            ((λ (($dog :: Entity))
+               (Bind
+                ($ctx3 :: (Referents Entity))
+                (Context)
+                (CloseClause
+                 (λ (($actual_event :: (Referents Eventuality)))
+                   (∧
+                    ((λ (($event :: (Referents Eventuality))) (tavla $dog $cats $ctx3 $event)) $actual_event)
+                    (fasnu $actual_event))))))
+             $member)))))))))
+  (case (id "31a52745397b69a3ab4672c18fa2d64ea75cc32a")
+    (status available)
+    (term
+     (SetOf
+      (λ (($z :: Entity))
+        (¬
+         (Bind
+          ($w1 :: (Referents Entity))
+          (SelectAtLeast 1 (λ (($x :: Entity)) (gerku $x)))
+          ((λ (($w :: (Referents Entity)))
+             (CloseClause
+              (λ (($actual_event :: (Referents Eventuality)))
+                (∧ ((λ (($event :: (Referents Eventuality))) (jmaji $w $event)) $actual_event) (fasnu $actual_event)))))
+           $w1)))))))
+  (case (id "33adac16a15100bdd23e72514dc4a78a96e70a6b")
+    (status unavailable)
+    (reason
+     "a0-expand-let: (a0-expand-let $a (Act Assertion) (Assert (CloseWith (row klama 5 direct-event (1 2 3 4 5)) ((1 Audience)))) (Bind (($o (ActOccurrence Assertion) (Perform Host $a))) (Do (Perform AttachedDisplay (Express (Close (Unhappiness Speaker $o Intense))))))) is not in my domain"))
+  (case (id "37da0499ed432c8b54b6d072a4b1c3852e9ad2df")
+    (status available)
+    (term
+     (Bind
+      ($w :: (Referents Entity))
+      (SelectExactly 3 (λ (($x :: Entity)) (gerku $x)))
+      (Assert
+       (Bind
+        ($ctx3 :: (Referents Entity))
+        (Context)
+        (CloseClause
+         (λ (($actual_event :: (Referents Eventuality)))
+           (∧
+            ((λ (($event :: (Referents Eventuality))) (tavla Speaker $w $ctx3 $event)) $actual_event)
+            (fasnu $actual_event)))))))))
+  (case (id "3948dd78d5112f473847359d17f681269520ce9f")
+    (status available)
+    (term
+     (Mention
+      (Bind
+       ($ctx2 :: (Referents Entity))
+       (Context)
+       ($ctx3 :: (Referents Entity))
+       (Context)
+       ($ctx4 :: (Referents Entity))
+       (Context)
+       ($ctx5 :: (Referents Entity))
+       (Context)
+       (CloseClause
+        (λ (($actual_event :: (Referents Eventuality)))
+          (∧
+           ((λ (($event :: (Referents Eventuality))) (klama Speaker $ctx2 $ctx3 $ctx4 $ctx5 $event)) $actual_event)
+           (fasnu $actual_event))))))))
+  (case (id "3956e1cb70c49637158cd4a7407ac5ccf982c17d")
+    (status available)
+    (term
+     (Bind
+      ($r :: (Referents Entity))
+      (Refer (λ (($unit :: (Referents Entity))) (mlatu $unit)))
+      (Assert
+       (CloseClause
+        (λ (($actual_event :: (Referents Eventuality)))
+          (∧ ((StateClause (blabi $r)) $actual_event) (fasnu $actual_event))))))))
+  (case (id "3adb0bedbd092a0ff9e28b5abeb9d81c14d69fb7")
+    (status available)
+    (term
+     (Bind
+      ($w :: (Referents Entity))
+      (SelectExactly 3 (λ (($x :: Entity)) (gerku $x)))
+      (Assert
+       (Bind
+        ($ctx3 :: (Referents Entity))
+        (Context)
+        (CloseClause
+         (λ (($actual_event :: (Referents Eventuality)))
+           (∧
+            ((λ (($event :: (Referents Eventuality))) (tavla $w Speaker $ctx3 $event)) $actual_event)
+            (fasnu $actual_event)))))))))
+  (case (id "4042ee2afc837aa8bea2a718993dd4ed719ad42d")
+    (status available)
+    (term
+     (Bind
+      ($r :: (PredTerm (Row (1 (Referents Entity)) (2 (Referents Entity)))))
+      (Context)
+      (Mention (Close ($r Speaker Audience))))))
+  (case (id "411ad460c5065d3e54df4217a226516cb9b7e4ea")
+    (status unavailable)
+    (reason
+     "b1-expand-some: (b1-expand-some Entity (λ (($x Entity)) (gerku $x)) (λ (($w (Referents Entity))) (Bind (($s Scale (Context))) (CloseWith (row jmaji 1 direct-event (1)) ((1 $w)))))) is not in my domain"))
+  (case (id "414f10bf35ddfae2fb13794f4f47e52537896503")
+    (status unavailable)
+    (reason
+     "b1-expand-select-some: (b1-expand-select-some Entity (λ (($x Entity)) (Bind (($s Scale (Context))) (gerku $x)))) is not in my domain"))
+  (case (id "425860a14d288938ee20bc473c86d3a5ce7f287b")
+    (status unavailable)
+    (reason
+     "b1-expand-every: (b1-expand-every Entity (λ (($x Entity)) (Bind (($s Scale (Context))) (gerku $x))) (λ (($x Entity)) (CloseWith (row jmaji 1 direct-event (1)) ((1 $x))))) is not in my domain"))
+  (case (id "428f277a9ec2c492ede935d0c890b996747f1a48")
+    (status available)
+    (term
+     (Assert
+      (Bind
+       ($w1 :: (Referents Entity))
+       (Presuppose
+        (∃ (λ (($x :: Entity)) (gerku $x)))
+        (Refer
+         (λ (($reference :: (Referents Entity)))
+           (∧
+            (∧
+             (∀ (λ (($member :: Entity)) (→ (Among $member $reference) ((λ (($x :: Entity)) (gerku $x)) $member))))
+             (∀
+              (λ (($subreference :: (Referents Entity)))
+                (→
+                 (Among $subreference $reference)
+                 (∃
+                  (λ (($member :: Entity))
+                    (∧
+                     ((λ (($x :: Entity)) (gerku $x)) $member)
+                     (∃
+                      (λ (($common :: (Referents Entity)))
+                        (∧ (Among $common $member) (Among $common $subreference)))))))))))
+            (∀ (λ (($member :: Entity)) (→ ((λ (($x :: Entity)) (gerku $x)) $member) (Among $member $reference))))))))
+       (∀
+        (λ (($member :: Entity))
+          (→
+           (Among $member $w1)
+           ((λ (($dog :: Entity))
+              (Bind
+               ($w1 :: (Referents Entity))
+               (SelectAtLeast 1 (λ (($y :: Entity)) (mlatu $y)))
+               ((λ (($w :: (Referents Entity)))
+                  (Bind
+                   ($ctx3 :: (Referents Entity))
+                   (Context)
+                   (CloseClause
+                    (λ (($actual_event :: (Referents Eventuality)))
+                      (∧
+                       ((λ (($event :: (Referents Eventuality))) (tavla $dog $w $ctx3 $event)) $actual_event)
+                       (fasnu $actual_event))))))
+                $w1)))
+            $member))))))))
+  (case (id "42c5da2578ee0adc173a7789faa03e92164665f5")
+    (status available)
+    (term
+     (λ (($p :: (Fn (Eventuality) Content)) ($c :: ClauseContent))
+       (Bind ($w :: (Referents Eventuality)) (SelectExactly 1 $p) ($c $w)))))
+  (case (id "433ec3111f68075021ba6c7dfe06b7b0621e2e0f")
+    (status unavailable)
+    (reason
+     "b1-expand-at-least: no clauses matched for (b1-expand-at-least $n Entity (λ (($x Entity)) (prenu $x)) (λ (($w (Referents Entity))) (CloseWith (row klama 5 direct-event (1 2 3 4 5)) ((1 $w)))))"))
+  (case (id "44e5b78b641625649b30470a6137d2e0f0c9f199")
+    (status available)
+    (term
+     (λ (($e :: (Referents Eventuality)))
+       (Bind
+        ($ctx2 :: (Referents Entity))
+        (Context)
+        ($ctx3 :: (Referents Entity))
+        (Context)
+        ($ctx4 :: (Referents Entity))
+        (Context)
+        ($ctx5 :: (Referents Entity))
+        (Context)
+        (CloseClause
+         (λ (($clause_event :: (Referents Eventuality)))
+           (∧
+            (∧ (Among $clause_event $e) (Among $e $clause_event))
+            ((λ (($actual_event :: (Referents Eventuality)))
+               (∧
+                ((λ (($lexical_event :: (Referents Eventuality)))
+                   (klama Speaker $ctx2 $ctx3 $ctx4 $ctx5 $lexical_event))
+                 $actual_event)
+                (fasnu $actual_event)))
+             $e))))))))
+  (case (id "4609d82730c3a0bb8c83f2db338169bafd034c35")
+    (status unavailable)
+    (reason
+     "b1-expand-at-least: no clauses matched for (b1-expand-at-least $n Entity (λ (($x Entity)) (gerku $x)) (λ (($w (Referents Entity))) (CloseWith (row tavla 3 direct-event (1 2 3)) ((1 Speaker) (2 $w)))))"))
+  (case (id "4852eeac9e86db4cb6d6d4a19469f720a7962e82")
+    (status available)
+    (term
+     (Assert
+      (Bind
+       ($w :: (Referents Entity))
+       (Presuppose
+        (∃ (λ (($x :: Entity)) (gerku $x)))
+        (Refer
+         (λ (($reference :: (Referents Entity)))
+           (∧
+            (∧
+             (∀ (λ (($member :: Entity)) (→ (Among $member $reference) ((λ (($x :: Entity)) (gerku $x)) $member))))
+             (∀
+              (λ (($subreference :: (Referents Entity)))
+                (→
+                 (Among $subreference $reference)
+                 (∃
+                  (λ (($member :: Entity))
+                    (∧
+                     ((λ (($x :: Entity)) (gerku $x)) $member)
+                     (∃
+                      (λ (($common :: (Referents Entity)))
+                        (∧ (Among $common $member) (Among $common $subreference)))))))))))
+            (∀ (λ (($member :: Entity)) (→ ((λ (($x :: Entity)) (gerku $x)) $member) (Among $member $reference))))))))
+       (∀
+        (λ (($member :: Entity))
+          (→
+           (Among $member $w)
+           ((λ (($x :: Entity))
+              (CloseClause
+               (λ (($actual_event :: (Referents Eventuality)))
+                 (∧ ((StateClause (blabi $x)) $actual_event) (fasnu $actual_event)))))
+            $member))))))))
+  (case (id "485f696c95709bf7fafedf22976a8763d63f5496")
+    (status available)
+    (term
+     (SetOf
+      (λ (($z :: Entity))
+        (¬
+         (Bind
+          ($w1 :: (Referents Entity))
+          (SelectAtLeast 1 (λ (($x :: Entity)) (gerku $x)))
+          ((λ (($w :: (Referents Entity)))
+             (CloseClause
+              (λ (($actual_event :: (Referents Eventuality)))
+                (∧ ((λ (($event :: (Referents Eventuality))) (jmaji $w $event)) $actual_event) (fasnu $actual_event)))))
+           $w1)))))))
+  (case (id "4955a8c68f8935068ee2677cd187fc98421260f7")
+    (status available)
+    (term
+     (SetOf
+      (λ (($z :: Entity))
+        (=
+         (Card
+          (SetOf
+           (λ (($global_member :: Entity))
+             (∧
+              ((λ (($x :: Entity)) (gerku $x)) $global_member)
+              ((λ (($x :: Entity))
+                 (CloseClause
+                  (λ (($actual_event :: (Referents Eventuality)))
+                    (∧
+                     ((λ (($event :: (Referents Eventuality))) (jmaji $x $event)) $actual_event)
+                     (fasnu $actual_event)))))
+               $global_member)))))
+         1)))))
+  (case (id "4cc6a45509151b5a0827ca4741f05c3e9e3afb8c")
+    (status available)
+    (term
+     (Bind
+      ($r :: (Referents Entity))
+      (Refer (λ (($unit :: (Referents Entity))) (gerku $unit)))
+      (Bind
+       ($ctx3 :: (Referents Entity))
+       (Context)
+       (CloseClause
+        (λ (($actual_event :: (Referents Eventuality)))
+          (∧
+           ((λ (($event :: (Referents Eventuality))) (tavla Speaker $r $ctx3 $event)) $actual_event)
+           (fasnu $actual_event))))))))
+  (case (id "4d4ad03ba86cacd6bea93987224d45d7ee5e94bc")
+    (status available)
+    (term
+     (Bind
+      ($w1 :: (Referents Entity))
+      (SelectAtLeast 1 (λ (($x :: Entity)) (gerku $x)))
+      ((λ (($w :: (Referents Entity)))
+         (Bind
+          ($ctx3 :: (Referents Entity))
+          (Context)
+          (CloseClause
+           (λ (($actual_event :: (Referents Eventuality)))
+             (∧
+              ((λ (($event :: (Referents Eventuality))) (tavla Speaker $w $ctx3 $event)) $actual_event)
+              (fasnu $actual_event))))))
+       $w1))))
+  (case (id "4dac43977fdeb1253b10b424e67c05ad70fea1f2")
+    (status available)
+    (term
+     (Bind
+      ($r :: (Referents Entity))
+      (Refer (λ (($unit :: (Referents Entity))) (gerku $unit)))
+      (Mention
+       (Bind
+        ($ctx3 :: (Referents Entity))
+        (Context)
+        (CloseClause
+         (λ (($actual_event :: (Referents Eventuality)))
+           (∧
+            ((λ (($event :: (Referents Eventuality))) (tavla Speaker $r $ctx3 $event)) $actual_event)
+            (fasnu $actual_event)))))))))
+  (case (id "4e062973565a461bfbff8b1c1e2b311b9849f16b")
+    (status available)
+    (term
+     (Assert
+      (Bind
+       ($ctx2 :: (Referents Entity))
+       (Context)
+       ($ctx3 :: (Referents Entity))
+       (Context)
+       (CloseClause
+        (λ (($actual_event :: (Referents Eventuality)))
+          (∧
+           ((λ (($event :: (Referents Eventuality))) (tavla Speaker $ctx2 $ctx3 $event)) $actual_event)
+           (fasnu $actual_event))))))))
+  (case (id "4e4c65ee9d06e77cf05541003764e803eb2f029a")
+    (status available)
+    (term
+     (Bind
+      ($ep :: (Referents Epistemology))
+      (Context)
+      (Bind
+       ($tv :: (Referents TruthValue))
+       (Refer
+        (λ (($v :: (Referents TruthValue)))
+          ((JeiRel
+            (Bind
+             ($ctx2 :: (Referents Entity))
+             (Context)
+             ($ctx3 :: (Referents Entity))
+             (Context)
+             ($ctx4 :: (Referents Entity))
+             (Context)
+             ($ctx5 :: (Referents Entity))
+             (Context)
+             (CloseClause
+              (λ (($actual_event :: (Referents Eventuality)))
+                (∧
+                 ((λ (($event :: (Referents Eventuality))) (klama Speaker $ctx2 $ctx3 $ctx4 $ctx5 $event))
+                  $actual_event)
+                 (fasnu $actual_event))))))
+           $v
+           $ep)))
+       (Mention $tv)))))
+  (case (id "4f89bfd19bf3d029272554a38f23f8f00d4c05fe")
+    (status available)
+    (term
+     (Bind
+      ($r :: (Referents Entity))
+      (Refer (λ (($unit1 :: (Referents Entity))) (mlatu $unit1)))
+      (Bind
+       ($r1 :: (Referents Entity))
+       (Refer (λ (($unit :: (Referents Entity))) (gerku $unit)))
+       (Assert
+        (Bind
+         ($ctx2 :: (Referents Entity))
+         (Context)
+         ($ctx4 :: (Referents Entity))
+         (Context)
+         ($ctx5 :: (Referents Entity))
+         (Context)
+         (CloseClause
+          (λ (($actual_event :: (Referents Eventuality)))
+            (∧
+             ((λ (($event :: (Referents Eventuality))) (klama $r1 $ctx2 $r $ctx4 $ctx5 $event)) $actual_event)
+             (fasnu $actual_event))))))))))
+  (case (id "5033153a5c5b68c485fe108ee8c910f18dd71434")
+    (status available)
+    (term
+     (Bind
+      ($r :: (Referents Entity))
+      (Refer (λ (($unit1 :: (Referents Entity))) (gerku $unit1)))
+      (Bind
+       ($r1 :: (Referents Entity))
+       (Refer (λ (($unit :: (Referents Entity))) (mlatu $unit)))
+       (Assert
+        (Bind
+         ($ctx3 :: (Referents Entity))
+         (Context)
+         (CloseClause
+          (λ (($actual_event :: (Referents Eventuality)))
+            (∧
+             ((λ (($event :: (Referents Eventuality))) (tavla $r1 $r $ctx3 $event)) $actual_event)
+             (fasnu $actual_event))))))))))
+  (case (id "50ef8b629c53200c229526eff8a75f8fba6b259b")
+    (status available)
+    (term
+     (Bind
+      ($r :: (Referents Entity))
+      (Refer (λ (($unit :: (Referents Entity))) (gerku $unit)))
+      (Assert
+       (Bind
+        ($ctx3 :: (Referents Entity))
+        (Context)
+        (CloseClause
+         (λ (($actual_event :: (Referents Eventuality)))
+           (∧
+            ((λ (($event :: (Referents Eventuality))) (tavla $r Speaker $ctx3 $event)) $actual_event)
+            (fasnu $actual_event)))))))))
+  (case (id "519c65d3104d364d4363ff8b27eecdec8abe7b27")
+    (status available)
+    (term
+     (Assert
+      (Bind
+       ($ctx2 :: (Referents Entity))
+       (Context)
+       ($ctx3 :: (Referents Entity))
+       (Context)
+       ($ctx4 :: (Referents Entity))
+       (Context)
+       ($ctx5 :: (Referents Entity))
+       (Context)
+       (CloseClause
+        (λ (($actual_event :: (Referents Eventuality)))
+          (∧
+           ((λ (($event :: (Referents Eventuality))) (klama Speaker $ctx2 $ctx3 $ctx4 $ctx5 $event)) $actual_event)
+           (fasnu $actual_event))))))))
+  (case (id "536aa8f5d8a23f0b5e51bf8b6b43a218c4634bcb")
+    (status unavailable)
+    (reason
+     "a0-expand-global-exactly: (a0-expand-global-exactly 1 Entity (λ (($x Entity)) (Bind (($s Scale (Context))) (gerku $x))) (λ (($x Entity)) (CloseWith (row jmaji 1 direct-event (1)) ((1 $x))))) is not in my domain"))
+  (case (id "53c6842442de071df126728dfc8a835ce2091e9b")
+    (status available)
+    (term
+     (Bind
+      ($dogs :: (Referents Entity))
+      (SelectExactly 3 (λ (($x :: Entity)) (gerku $x)))
+      ($people :: (Referents Entity))
+      (SelectExactly 2 (λ (($x :: Entity)) (prenu $x)))
+      (Assert
+       (∀
+        (λ (($member :: Entity))
+          (→
+           (Among $member $dogs)
+           ((λ (($d :: Entity))
+              (∀
+               (λ (($member :: Entity))
+                 (→
+                  (Among $member $people)
+                  ((λ (($p :: Entity))
+                     (CloseClause
+                      (λ (($actual_event :: (Referents Eventuality)))
+                        (∧ ((StateClause (nelci $d $p)) $actual_event) (fasnu $actual_event)))))
+                   $member)))))
+            $member))))))))
+  (case (id "58c16dbd8c5ab4d9d247b7053a082b392b277d90")
+    (status unavailable)
+    (reason
+     "b1-expand-no: (b1-expand-no Entity (λ (($x Entity)) (gerku $x)) (λ (($w (Referents Entity))) (Bind (($s Scale (Context))) (CloseWith (row jmaji 1 direct-event (1)) ((1 $w)))))) is not in my domain"))
+  (case (id "5adee1115a50ccc807e02297198c6d2c11bb1ea9")
+    (status available)
+    (term
+     (Assert
+      (Bind
+       ($w1 :: (Referents Entity))
+       (SelectAtLeast 1 (λ (($x :: Entity)) (gerku $x)))
+       ((λ (($w :: (Referents Entity)))
+          (Bind
+           ($ctx3 :: (Referents Entity))
+           (Context)
+           (CloseClause
+            (λ (($actual_event :: (Referents Eventuality)))
+              (∧
+               ((λ (($event :: (Referents Eventuality))) (tavla $w Speaker $ctx3 $event)) $actual_event)
+               (fasnu $actual_event))))))
+        $w1)))))
+  (case (id "5b327dd7decfabf290e971fdee6123a55d5c4d26")
+    (status available)
+    (term
+     (Assert
+      (CloseClause
+       (λ (($actual_event :: (Referents Eventuality)))
+         (∧
+          ((λ (($event :: (Referents Eventuality))) (jmaji (Combine Speaker Audience) $event)) $actual_event)
+          (fasnu $actual_event)))))))
+  (case (id "5ce3bc7019740c791f9acdfc644d21e92d62dcb7")
+    (status unavailable)
+    (reason
+     "a0-expand-close: (a0-expand-close (row valsi 2 holding-state (1 2)) ((1 (WordSign klama)))) is not in my domain"))
+  (case (id "5f5b053a4dcccf2858daa126fd3d854e0e78d516")
+    (status available)
+    (term
+     (∧
+      ((λ (($s :: (Referents Entity)) ($l :: (Referents Entity)))
+         (Bind
+          ($ctx3 :: (Referents Entity))
+          (Context)
+          (CloseClause
+           (λ (($actual_event :: (Referents Eventuality)))
+             (∧
+              ((λ (($event :: (Referents Eventuality))) (tavla $s $l $ctx3 $event)) $actual_event)
+              (fasnu $actual_event))))))
+       Speaker
+       Audience)
+      (∧
+       ((λ (($s :: (Referents Entity)) ($l :: (Referents Entity)))
+          (Bind
+           ($ctx3 :: (Referents Entity))
+           (Context)
+           (CloseClause
+            (λ (($actual_event :: (Referents Eventuality)))
+              (∧
+               ((λ (($event :: (Referents Eventuality))) (tavla $s $l $ctx3 $event)) $actual_event)
+               (fasnu $actual_event))))))
+        Audience
+        Speaker)
+       (∧)))))
+  (case (id "5fb2cbaf51ee51ea8e04140f1410110e6f30ccbf")
+    (status available)
+    (term
+     (Bind
+      ($kind :: (Referents Eventuality))
+      (Refer (λ (($k :: (Referents Eventuality))) (fasnu $k)))
+      (Bind
+       ($a :: (Referents AbstractNature))
+       (Refer
+        (λ (($x :: (Referents AbstractNature)))
+          (Close
+           ((SuhuRel
+             (Bind
+              ($ctx2 :: (Referents Entity))
+              (Context)
+              ($ctx3 :: (Referents Entity))
+              (Context)
+              ($ctx4 :: (Referents Entity))
+              (Context)
+              ($ctx5 :: (Referents Entity))
+              (Context)
+              (CloseClause
+               (λ (($actual_event :: (Referents Eventuality)))
+                 (∧
+                  ((λ (($event :: (Referents Eventuality))) (klama Speaker $ctx2 $ctx3 $ctx4 $ctx5 $event))
+                   $actual_event)
+                  (fasnu $actual_event))))))
+            $x
+            $kind))))
+       (Mention $a)))))
+  (case (id "5feeebff2d1f37decc454689cbde025cfd011b4a")
+    (status available)
+    (term
+     (Assert
+      (Bind
+       ($w :: (Referents Entity))
+       (Presuppose
+        (∃ (λ (($x :: Entity)) (gerku $x)))
+        (Refer
+         (λ (($reference :: (Referents Entity)))
+           (∧
+            (∧
+             (∀ (λ (($member :: Entity)) (→ (Among $member $reference) ((λ (($x :: Entity)) (gerku $x)) $member))))
+             (∀
+              (λ (($subreference :: (Referents Entity)))
+                (→
+                 (Among $subreference $reference)
+                 (∃
+                  (λ (($member :: Entity))
+                    (∧
+                     ((λ (($x :: Entity)) (gerku $x)) $member)
+                     (∃
+                      (λ (($common :: (Referents Entity)))
+                        (∧ (Among $common $member) (Among $common $subreference)))))))))))
+            (∀ (λ (($member :: Entity)) (→ ((λ (($x :: Entity)) (gerku $x)) $member) (Among $member $reference))))))))
+       (∀
+        (λ (($member :: Entity))
+          (→
+           (Among $member $w)
+           ((λ (($x :: Entity))
+              (Bind
+               ($nuclear_tavla_3 :: (Referents Entity))
+               (Context)
+               (=
+                (Card
+                 (SetOf
+                  (λ (($global_member :: Entity))
+                    (∧
+                     ((λ (($restrictor_member :: Entity)) (mlatu $restrictor_member)) $global_member)
+                     ((λ (($nuclear_member :: Entity))
+                        (CloseClause
+                         (λ (($actual_event :: (Referents Eventuality)))
+                           (∧
+                            ((λ (($event :: (Referents Eventuality)))
+                               (tavla $x $nuclear_member $nuclear_tavla_3 $event))
+                             $actual_event)
+                            (fasnu $actual_event)))))
+                      $global_member)))))
+                3)))
+            $member))))))))
+  (case (id "60e32117d888221df45163e11f73a0509649fe93")
+    (status available)
+    (term
+     (Mention
+      (Bind
+       ($w1 :: (Referents Entity))
+       (SelectAtLeast 1 (λ (($x :: Entity)) (gerku $x)))
+       ((λ (($w :: (Referents Entity)))
+          (Bind
+           ($ctx3 :: (Referents Entity))
+           (Context)
+           (CloseClause
+            (λ (($actual_event :: (Referents Eventuality)))
+              (∧
+               ((λ (($event :: (Referents Eventuality))) (tavla Speaker $w $ctx3 $event)) $actual_event)
+               (fasnu $actual_event))))))
+        $w1)))))
+  (case (id "622e4a564152b3e60db8afdd669d462b46663afe")
+    (status available)
+    (term
+     (Bind
+      ($r :: (Referents Entity))
+      (Refer (λ (($unit :: (Referents Entity))) (mlatu $unit)))
+      (Assert
+       (Bind
+        ($w :: (Referents Entity))
+        (Presuppose
+         (∃ (λ (($x :: Entity)) (gerku $x)))
+         (Refer
+          (λ (($reference :: (Referents Entity)))
+            (∧
+             (∧
+              (∀ (λ (($member :: Entity)) (→ (Among $member $reference) ((λ (($x :: Entity)) (gerku $x)) $member))))
+              (∀
+               (λ (($subreference :: (Referents Entity)))
+                 (→
+                  (Among $subreference $reference)
+                  (∃
+                   (λ (($member :: Entity))
+                     (∧
+                      ((λ (($x :: Entity)) (gerku $x)) $member)
+                      (∃
+                       (λ (($common :: (Referents Entity)))
+                         (∧ (Among $common $member) (Among $common $subreference)))))))))))
+             (∀ (λ (($member :: Entity)) (→ ((λ (($x :: Entity)) (gerku $x)) $member) (Among $member $reference))))))))
+        (∀
+         (λ (($member :: Entity))
+           (→
+            (Among $member $w)
+            ((λ (($x :: Entity))
+               (Bind
+                ($ctx3 :: (Referents Entity))
+                (Context)
+                (CloseClause
+                 (λ (($actual_event :: (Referents Eventuality)))
+                   (∧
+                    ((λ (($event :: (Referents Eventuality))) (tavla $x $r $ctx3 $event)) $actual_event)
+                    (fasnu $actual_event))))))
+             $member)))))))))
+  (case (id "635a3aa7bafa3719cc67c19e9d139aacb53252c0")
+    (status available)
+    (term
+     (Bind
+      ($r :: (Referents Entity))
+      (Refer (λ (($unit :: (Referents Entity))) (mlatu $unit)))
+      (Assert
+       (¬
+        (Bind
+         ($w1 :: (Referents Entity))
+         (SelectAtLeast 1 (λ (($x :: Entity)) (gerku $x)))
+         ((λ (($w :: (Referents Entity)))
+            (Bind
+             ($ctx3 :: (Referents Entity))
+             (Context)
+             (CloseClause
+              (λ (($actual_event :: (Referents Eventuality)))
+                (∧
+                 ((λ (($event :: (Referents Eventuality))) (tavla $r $w $ctx3 $event)) $actual_event)
+                 (fasnu $actual_event))))))
+          $w1)))))))
+  (case (id "6489b84bf8e9ceae95a45d0dc9a4bed9e4eb6514")
+    (status available)
+    (term
+     (Bind
+      ($r :: (Referents Entity))
+      (Refer (λ (($unit :: (Referents Entity))) (mlatu $unit)))
+      (Bind
+       ($nuclear_tavla_3 :: (Referents Entity))
+       (Context)
+       (Assert
+        (=
+         (Card
+          (SetOf
+           (λ (($global_member :: Entity))
+             (∧
+              ((λ (($restrictor_member :: Entity)) (gerku $restrictor_member)) $global_member)
+              ((λ (($nuclear_member :: Entity))
+                 (CloseClause
+                  (λ (($actual_event :: (Referents Eventuality)))
+                    (∧
+                     ((λ (($event :: (Referents Eventuality))) (tavla $nuclear_member $r $nuclear_tavla_3 $event))
+                      $actual_event)
+                     (fasnu $actual_event)))))
+               $global_member)))))
+         3))))))
+  (case (id "64c15957e568587d74aa30b873ef5aa684436258")
+    (status available)
+    (term
+     (Bind
+      ($r :: (Referents Entity))
+      (Refer (λ (($unit2 :: (Referents Entity))) (prenu $unit2)))
+      (Bind
+       ($r1 :: (Referents Entity))
+       (Refer (λ (($unit1 :: (Referents Entity))) (gerku $unit1)))
+       (Bind
+        ($r2 :: (Referents Entity))
+        (Refer (λ (($unit :: (Referents Entity))) (mlatu $unit)))
+        (Assert
+         (Bind
+          ($ctx4 :: (Referents Entity))
+          (Context)
+          ($ctx5 :: (Referents Entity))
+          (Context)
+          (CloseClause
+           (λ (($actual_event :: (Referents Eventuality)))
+             (∧
+              ((λ (($event :: (Referents Eventuality))) (klama $r $r1 $r2 $ctx4 $ctx5 $event)) $actual_event)
+              (fasnu $actual_event)))))))))))
+  (case (id "6584fc7110a48d8b01400f0fed7714f08cf3cbac")
+    (status unavailable)
+    (reason
+     "a0-expand-exactly: (a0-expand-exactly 0 Entity (λ (($x Entity)) (gerku $x)) (λ (($w (Referents Entity))) (Bind (($s Scale (Context))) (CloseWith (row jmaji 1 direct-event (1)) ((1 $w)))))) is not in my domain"))
+  (case (id "661c26cadee3dc745ccebb82394c046d78ee79a7")
+    (status available)
+    (term
+     (Bind
+      ($r :: (Referents Entity))
+      (Refer (λ (($unit1 :: (Referents Entity))) (gerku $unit1)))
+      (Bind
+       ($r1 :: (Referents Entity))
+       (Refer (λ (($unit :: (Referents Entity))) (gerku $unit)))
+       (Assert
+        (Bind
+         ($ctx3 :: (Referents Entity))
+         (Context)
+         (CloseClause
+          (λ (($actual_event :: (Referents Eventuality)))
+            (∧
+             ((λ (($event :: (Referents Eventuality))) (tavla $r $r1 $ctx3 $event)) $actual_event)
+             (fasnu $actual_event))))))))))
+  (case (id "676aca15433b25852f0cb06540b381890f0b57a6")
+    (status available)
+    (term
+     (Assert
+      (CloseClause
+       (λ (($actual_event :: (Referents Eventuality)))
+         (∧ ((StateClause (remna (Combine Speaker Audience))) $actual_event) (fasnu $actual_event)))))))
+  (case (id "68d76ee28c33ecdc9d3ddeebc06340e47b086fc9")
+    (status available)
+    (term
+     (SetOf
+      (λ (($z :: Entity))
+        (¬
+         (Bind
+          ($w1 :: (Referents Entity))
+          (SelectAtLeast 1 (λ (($x :: Entity)) (gerku $x)))
+          ((λ (($w :: (Referents Entity)))
+             (CloseClause
+              (λ (($actual_event :: (Referents Eventuality)))
+                (∧ ((λ (($event :: (Referents Eventuality))) (jmaji $w $event)) $actual_event) (fasnu $actual_event)))))
+           $w1)))))))
+  (case (id "6acd3321836246a9a199a76f55d4d3e00e681762")
+    (status available)
+    (term
+     (Bind
+      ($r :: (Referents Entity))
+      (Refer (λ (($named :: (Referents Entity))) (Named "alis" $named)))
+      (Assert
+       (Bind
+        ($ctx3 :: (Referents Entity))
+        (Context)
+        (CloseClause
+         (λ (($actual_event :: (Referents Eventuality)))
+           (∧
+            ((λ (($event :: (Referents Eventuality))) (tavla Speaker $r $ctx3 $event)) $actual_event)
+            (fasnu $actual_event)))))))))
+  (case (id "6b708ddcdacf0a49ffaf55306f0cccad98046a67")
+    (status available)
+    (term
+     (Bind
+      ($purpose :: (Referents Entity))
+      (Context)
+      ($n :: Natural)
+      (Vague (AdmissibleThreshold TooManyK (λ (($x :: Entity)) (gerku $x)) $purpose))
+      (Assert
+       (Bind
+        ($w1 :: (Referents Entity))
+        (SelectAtLeast (+ $n 1) (λ (($x :: Entity)) (gerku $x)))
+        ((λ (($w :: (Referents Entity)))
+           (Bind
+            ($ctx3 :: (Referents Entity))
+            (Context)
+            (CloseClause
+             (λ (($actual_event :: (Referents Eventuality)))
+               (∧
+                ((λ (($event :: (Referents Eventuality))) (tavla Speaker $w $ctx3 $event)) $actual_event)
+                (fasnu $actual_event))))))
+         $w1))))))
+  (case (id "6db1d0ab2a56d4dec895dc6191ac5bc37881bc41")
+    (status available)
+    (term
+     (Bind
+      ($base :: (Referents Entity))
+      (Local (Refer (λ (($x :: Entity)) (gerku $x))))
+      (Bind
+       ($sets :: (Referents (Set Entity)))
+       (Refer
+        (λ (($s :: (Set Entity)))
+          (CloseClause
+           (λ (($actual_event :: (Referents Eventuality)))
+             (∧ ((StateClause (selcmi $s $base)) $actual_event) (fasnu $actual_event))))))
+       (Mention $sets)))))
+  (case (id "6dda66c58218158e235fe50e2f640eb4570dc8d9")
+    (status available)
+    (term
+     (Bind
+      ($w1 :: (Referents Entity))
+      (SelectAtLeast 1 (λ (($x :: Entity)) (gerku $x)))
+      ((λ (($w :: (Referents Entity)))
+         (Bind
+          ($ctx3 :: (Referents Entity))
+          (Context)
+          (CloseClause
+           (λ (($actual_event :: (Referents Eventuality)))
+             (∧
+              ((λ (($event :: (Referents Eventuality))) (tavla $w Speaker $ctx3 $event)) $actual_event)
+              (fasnu $actual_event))))))
+       $w1))))
+  (case (id "6e39ed994d886bf1029e9d81b13d2c4969d12f1c")
+    (status available)
+    (term
+     (SetOf
+      (λ (($z :: Entity))
+        (¬
+         (Bind
+          ($w1 :: (Referents Entity))
+          (SelectAtLeast (+ 1 1) (λ (($x :: Entity)) (gerku $x)))
+          ((λ (($w :: (Referents Entity)))
+             (CloseClause
+              (λ (($actual_event :: (Referents Eventuality)))
+                (∧ ((λ (($event :: (Referents Eventuality))) (jmaji $w $event)) $actual_event) (fasnu $actual_event)))))
+           $w1)))))))
+  (case (id "6e60ee9760e47fd7461b482efbc63e5c17e28444")
+    (status unavailable)
+    (reason
+     "a0-expand-let: (a0-expand-let $a (Act Assertion) (Assert (CloseWith (row klama 5 direct-event (1 2 3 4 5)) ((1 Audience)))) (Bind (($o (ActOccurrence Assertion) (Perform Host $a))) (Do (Perform AttachedDisplay (Express (Close (Happiness Speaker $o Moderate))))))) is not in my domain"))
+  (case (id "6ecb067d1e11340ae795c26b66ed1936248998a6")
+    (status available)
+    (term
+     (Bind
+      ($r :: (Referents Entity))
+      (Refer (λ (($named :: (Referents Entity))) (Named "alis" $named)))
+      (Assert
+       (Bind
+        ($w1 :: (Referents Entity))
+        (SelectExactly 3 (λ (($x :: Entity)) (gerku $x)))
+        ((λ (($w :: (Referents Entity)))
+           (Bind
+            ($ctx3 :: (Referents Entity))
+            (Context)
+            (CloseClause
+             (λ (($actual_event :: (Referents Eventuality)))
+               (∧
+                ((λ (($event :: (Referents Eventuality))) (tavla $w $r $ctx3 $event)) $actual_event)
+                (fasnu $actual_event))))))
+         $w1))))))
+  (case (id "6f6172a19fbd27927333f4dd1fa4152e9a5ae5c8")
+    (status unavailable)
+    (reason
+     "a0-expand-let: (a0-expand-let $a1 (Act Assertion) (Assert (CloseWith (row klama 5 direct-event (1 2 3 4 5)) ((1 Speaker)))) (Bind (($o1 (ActOccurrence Assertion) (Perform Host $a1))) (Let ($a2 (Act Assertion)) (Assert (CloseWith (row stali 1 direct-event (1)) ((1 Audience)))) (Bind (($o2 (ActOccurrence Assertion) (Perform Host $a2))) (Do (Perform AttachedDisplay (Express (Close (Contrast $o2 $o1))))))))) is not in my domain"))
+  (case (id "6f7179b2bc813a079360002fde1531d22f13075a")
+    (status available)
+    (term
+     (SetOf
+      (λ (($z :: Entity))
+        (Bind
+         ($w :: (Referents Entity))
+         (Presuppose
+          (∃ (λ (($x :: Entity)) (gerku $x)))
+          (Refer
+           (λ (($reference :: (Referents Entity)))
+             (∧
+              (∧
+               (∀ (λ (($member :: Entity)) (→ (Among $member $reference) ((λ (($x :: Entity)) (gerku $x)) $member))))
+               (∀
+                (λ (($subreference :: (Referents Entity)))
+                  (→
+                   (Among $subreference $reference)
+                   (∃
+                    (λ (($member :: Entity))
+                      (∧
+                       ((λ (($x :: Entity)) (gerku $x)) $member)
+                       (∃
+                        (λ (($common :: (Referents Entity)))
+                          (∧ (Among $common $member) (Among $common $subreference)))))))))))
+              (∀ (λ (($member :: Entity)) (→ ((λ (($x :: Entity)) (gerku $x)) $member) (Among $member $reference))))))))
+         (∀
+          (λ (($member :: Entity))
+            (→
+             (Among $member $w)
+             ((λ (($x :: Entity))
+                (CloseClause
+                 (λ (($actual_event :: (Referents Eventuality)))
+                   (∧
+                    ((λ (($event :: (Referents Eventuality))) (jmaji $x $event)) $actual_event)
+                    (fasnu $actual_event)))))
+              $member)))))))))
+  (case (id "7093b728d78697d97257006327e2dcbdb9a365aa")
+    (status available)
+    (term
+     (Bind
+      ($restrictor_klama_2 :: (Referents Entity))
+      (Context)
+      ($restrictor_klama_3 :: (Referents Entity))
+      (Context)
+      ($restrictor_klama_4 :: (Referents Entity))
+      (Context)
+      ($restrictor_klama_5 :: (Referents Entity))
+      (Context)
+      ($nuclear_klama_2 :: (Referents Entity))
+      (Context)
+      ($nuclear_klama_3 :: (Referents Entity))
+      (Context)
+      ($nuclear_klama_4 :: (Referents Entity))
+      (Context)
+      ($nuclear_klama_5 :: (Referents Entity))
+      (Context)
+      (=
+       (Card
+        (SetOf
+         (λ (($global_member :: Entity))
+           (∧
+            ((λ (($restrictor_member :: Entity))
+               (CloseClause
+                (λ (($actual_event :: (Referents Eventuality)))
+                  (∧
+                   ((λ (($event :: (Referents Eventuality)))
+                      (klama
+                       $restrictor_member
+                       $restrictor_klama_2
+                       $restrictor_klama_3
+                       $restrictor_klama_4
+                       $restrictor_klama_5
+                       $event))
+                    $actual_event)
+                   (fasnu $actual_event)))))
+             $global_member)
+            ((λ (($nuclear_member :: Entity))
+               (CloseClause
+                (λ (($actual_event :: (Referents Eventuality)))
+                  (∧
+                   ((λ (($event :: (Referents Eventuality)))
+                      (klama
+                       $nuclear_member
+                       $nuclear_klama_2
+                       $nuclear_klama_3
+                       $nuclear_klama_4
+                       $nuclear_klama_5
+                       $event))
+                    $actual_event)
+                   (fasnu $actual_event)))))
+             $global_member)))))
+       3))))
+  (case (id "70d243e3fab7fa6f6e9075898b0883efc9ac6a64")
+    (status available)
+    (term
+     (Bind
+      ($cat :: (Referents Entity))
+      (Refer (λ (($x :: (Referents Entity))) (mlatu $x)))
+      (Do
+       (Assert
+        (CloseClause
+         (λ (($actual_event :: (Referents Eventuality)))
+           (∧ ((StateClause (blabi $cat)) $actual_event) (fasnu $actual_event)))))
+       (Assert
+        (Bind
+         ($ctx2 :: (Referents Entity))
+         (Context)
+         ($ctx3 :: (Referents Entity))
+         (Context)
+         (CloseClause
+          (λ (($actual_event :: (Referents Eventuality)))
+            (∧
+             ((λ (($event :: (Referents Eventuality))) (jbena $cat $ctx2 $ctx3 $event)) $actual_event)
+             (fasnu $actual_event))))))))))
+  (case (id "7318097d39a3fd427b8496b52e0a9c8c908bd088")
+    (status available)
+    (term
+     (λ (($p :: (EFn (Entity) Content)) ($r :: (Referents Entity)))
+       (∧
+        (∀ (λ (($member :: Entity)) (→ (Among $member $r) ($p $member))))
+        (∀
+         (λ (($subreference :: (Referents Entity)))
+           (→
+            (Among $subreference $r)
+            (∃
+             (λ (($member :: Entity))
+               (∧
+                ($p $member)
+                (∃
+                 (λ (($common :: (Referents Entity)))
+                   (∧ (Among $common $member) (Among $common $subreference))))))))))))))
+  (case (id "7489629dc458e9a2b37b77e7009276d086528421")
+    (status unavailable)
+    (reason
+     "b1-expand-more-than: (b1-expand-more-than 1 Entity (λ (($x Entity)) (gerku $x)) (λ (($w (Referents Entity))) (Bind (($s Scale (Context))) (CloseWith (row jmaji 1 direct-event (1)) ((1 $w)))))) is not in my domain"))
+  (case (id "7668b7e50f1b89af8fbe18ec31f6edbc45b1168c")
+    (status available)
+    (term
+     (Assert
+      (Generic
+       Typical
+       (λ (($x :: Entity)) (mlatu $x))
+       (λ (($x :: Entity))
+         (Bind
+          ($ctx2 :: (Referents Entity))
+          (Context)
+          (CloseClause
+           (λ (($actual_event :: (Referents Eventuality)))
+             (∧ ((StateClause (cinri $x $ctx2)) $actual_event) (fasnu $actual_event))))))))))
+  (case (id "7867eb120b34ea3b161cbf57dc7c72375822f193")
+    (status available)
+    (term
+     (Presuppose
+      (∃
+       (λ (($x :: Entity))
+         (∧
+          (prenu $x)
+          (∃
+           (λ (($y :: Entity))
+             (∧
+              (xasli $y)
+              (CloseClause
+               (λ (($actual_event :: (Referents Eventuality)))
+                 (∧ ((StateClause (ponse $x $y)) $actual_event) (fasnu $actual_event))))))))))
+      (∀
+       (λ (($p :: Entity) ($d :: (Referents Entity)))
+         (→
+          (∧
+           (prenu $p)
+           (∀ (λ (($member :: Entity)) (→ (Among $member $d) ((λ (($z :: Entity)) (xasli $z)) $member))))
+           (CloseClause
+            (λ (($actual_event :: (Referents Eventuality)))
+              (∧ ((StateClause (ponse $p $d)) $actual_event) (fasnu $actual_event)))))
+          (Bind
+           ($ctx3 :: (Referents Entity))
+           (Context)
+           (CloseClause
+            (λ (($actual_event :: (Referents Eventuality)))
+              (∧
+               ((λ (($event :: (Referents Eventuality))) (darxi $p $d $ctx3 $event)) $actual_event)
+               (fasnu $actual_event)))))))))))
+  (case (id "7cccf0a9acae76bbd8db11b56c25879603ef4cff") (status available) (term (SetOf (λ (($z :: Entity)) (∧)))))
+  (case (id "7d1e0a45041ecaa91bb99f88da953e476b218b8f")
+    (status available)
+    (term
+     (λ (($bread :: (Referents Entity)) ($breadUnit :: (Fn (Entity) Content)))
+       (∧
+        (∧
+         (∀ (λ (($member :: Entity)) (→ (Among $member $bread) ($breadUnit $member))))
+         (∀
+          (λ (($subreference :: (Referents Entity)))
+            (→
+             (Among $subreference $bread)
+             (∃
+              (λ (($member :: Entity))
+                (∧
+                 ($breadUnit $member)
+                 (∃
+                  (λ (($common :: (Referents Entity)))
+                    (∧ (Among $common $member) (Among $common $subreference)))))))))))
+        (∀
+         (λ (($r :: (Referents Entity)))
+           (→ (Among $r $bread) (∃ (λ (($s :: (Referents Entity))) (∧ (Among $s $r) (¬ (Among $r $s))))))))))))
+  (case (id "7f097098e1315809937f245c79749a84701de106")
+    (status available)
+    (term
+     (Generic
+      Typical
+      (λ (($x :: Entity)) (gerku $x))
+      (λ (($x :: Entity))
+        (Bind
+         ($s :: Scale)
+         (Context)
+         (CloseClause
+          (λ (($actual_event :: (Referents Eventuality)))
+            (∧ ((λ (($event :: (Referents Eventuality))) (jmaji $x $event)) $actual_event) (fasnu $actual_event)))))))))
+  (case (id "7f203497c357df2c9869f79e1b4eaa87c6c9de1c")
+    (status available)
+    (term
+     (Combine
+      Speaker
+      (CloseClause
+       (λ (($actual_event :: (Referents Eventuality)))
+         (∧ ((StateClause (gerku Speaker)) $actual_event) (fasnu $actual_event)))))))
+  (case (id "8061585a4f66d8b8e88b791afd3e6ad31da2df53")
+    (status available)
+    (term
+     (Bind
+      ($r :: (Referents Entity))
+      (Refer (λ (($unit :: (Referents Entity))) (mlatu $unit)))
+      (Assert
+       (Bind
+        ($w1 :: (Referents Entity))
+        (SelectExactly 3 (λ (($x :: Entity)) (gerku $x)))
+        ((λ (($w :: (Referents Entity)))
+           (Bind
+            ($ctx3 :: (Referents Entity))
+            (Context)
+            (CloseClause
+             (λ (($actual_event :: (Referents Eventuality)))
+               (∧
+                ((λ (($event :: (Referents Eventuality))) (tavla $r $w $ctx3 $event)) $actual_event)
+                (fasnu $actual_event))))))
+         $w1))))))
+  (case (id "808a6f9bdbbb1073dda1dc3a393dee0026919d4f")
+    (status available)
+    (term
+     (Bind
+      ($restrictor_klama_2 :: (Referents Entity))
+      (Context)
+      ($restrictor_klama_3 :: (Referents Entity))
+      (Context)
+      ($restrictor_klama_4 :: (Referents Entity))
+      (Context)
+      ($restrictor_klama_5 :: (Referents Entity))
+      (Context)
+      ($nuclear_bajra_2 :: (Referents Entity))
+      (Context)
+      ($nuclear_bajra_3 :: (Referents Entity))
+      (Context)
+      ($nuclear_bajra_4 :: (Referents Entity))
+      (Context)
+      (=
+       (Card
+        (SetOf
+         (λ (($global_member :: Entity))
+           (∧
+            ((λ (($restrictor_member :: Entity))
+               (CloseClause
+                (λ (($actual_event :: (Referents Eventuality)))
+                  (∧
+                   ((λ (($event :: (Referents Eventuality)))
+                      (klama
+                       $restrictor_member
+                       $restrictor_klama_2
+                       $restrictor_klama_3
+                       $restrictor_klama_4
+                       $restrictor_klama_5
+                       $event))
+                    $actual_event)
+                   (fasnu $actual_event)))))
+             $global_member)
+            ((λ (($nuclear_member :: Entity))
+               (CloseClause
+                (λ (($actual_event :: (Referents Eventuality)))
+                  (∧
+                   ((λ (($event :: (Referents Eventuality)))
+                      (bajra $nuclear_member $nuclear_bajra_2 $nuclear_bajra_3 $nuclear_bajra_4 $event))
+                    $actual_event)
+                   (fasnu $actual_event)))))
+             $global_member)))))
+       3))))
+  (case (id "80b377eeaeeff358d3b8c1f73fd2749ffb17cb57")
+    (status unavailable)
+    (reason
+     "a0-expand-exactly: (a0-expand-exactly 1 Entity (λ (($x Entity)) (gerku $x)) (λ (($w (Referents Entity))) (Bind (($s Scale (Context))) (CloseWith (row jmaji 1 direct-event (1)) ((1 $w)))))) is not in my domain"))
+  (case (id "81d3fa49e84bfcf00813d35fad8d70b23b8d3935")
+    (status available)
+    (term
+     (=
+      (Card
+       (SetOf
+        (λ (($global_member :: Entity))
+          (∧
+           ((λ (($x :: Entity)) (gerku $x)) $global_member)
+           ((λ (($x :: Entity))
+              (CloseClause
+               (λ (($actual_event :: (Referents Eventuality)))
+                 (∧
+                  ((λ (($event :: (Referents Eventuality))) (jmaji $x $event)) $actual_event)
+                  (fasnu $actual_event)))))
+            $global_member)))))
+      1)))
+  (case (id "8360021fa7e50952cd0f155fbb5c8ea9a845b60f")
+    (status available)
+    (term
+     (SentenceSign
+      (CloseClause
+       (λ (($actual_event :: (Referents Eventuality)))
+         (∧ ((StateClause (gerku Speaker)) $actual_event) (fasnu $actual_event)))))))
+  (case (id "8447f6258b31394149ce313493c037835dfbdc08")
+    (status available)
+    (term
+     (=
+      (Card
+       (SetOf
+        (λ (($global_member :: Entity))
+          (∧ ((λ (($p :: Entity)) (prenu $p)) $global_member) ((λ (($q :: Entity)) (blabi $q)) $global_member)))))
+      2)))
+  (case (id "84d3f3f5db6d9bb097e9df301673052e73e0649a")
+    (status available)
+    (term
+     (SetOf
+      (λ (($x :: Entity))
+        (Bind ($r :: (Referents Entity)) (SelectAtLeast 1 (λ (($y :: Entity)) (gerku $y))) (gerku $x))))))
+  (case (id "8ccd154413e727b9b34e8a038b034866944e530b")
+    (status unavailable)
+    (reason
+     "b1-expand-at-least: no clauses matched for (b1-expand-at-least $n Entity (λ (($x Entity)) (gerku $x)) (λ (($w (Referents Entity))) (CloseWith (row tavla 3 direct-event (1 2 3)) ((1 $w) (2 $r)))))"))
+  (case (id "8e1fab41bbb56ee118edf789bec2b290dedfaa2e")
+    (status unavailable)
+    (reason
+     "b1-expand-more-than: (b1-expand-more-than 1 Entity (λ (($x Entity)) (Bind (($s Scale (Context))) (gerku $x))) (λ (($w (Referents Entity))) (CloseWith (row jmaji 1 direct-event (1)) ((1 $w))))) is not in my domain"))
+  (case (id "90ea9f4b3bd16e1989e5d78f7db1bfc8698c46bd")
+    (status available)
+    (term
+     (Bind
+      ($nuclear_bajra_2 :: (Referents Entity))
+      (Context)
+      ($nuclear_bajra_3 :: (Referents Entity))
+      (Context)
+      ($nuclear_bajra_4 :: (Referents Entity))
+      (Context)
+      (Assert
+       (=
+        (Card
+         (SetOf
+          (λ (($global_member :: Entity))
+            (∧
+             ((λ (($restrictor_member :: Entity)) (gerku $restrictor_member)) $global_member)
+             ((λ (($nuclear_member :: Entity))
+                (CloseClause
+                 (λ (($actual_event :: (Referents Eventuality)))
+                   (∧
+                    ((λ (($event :: (Referents Eventuality)))
+                       (bajra $nuclear_member $nuclear_bajra_2 $nuclear_bajra_3 $nuclear_bajra_4 $event))
+                     $actual_event)
+                    (fasnu $actual_event)))))
+              $global_member)))))
+        3)))))
+  (case (id "94cf88a0926fcd3b3ed426e8325e749edea9ed95")
+    (status unavailable)
+    (reason
+     "b1-expand-at-least: (b1-expand-at-least 1 Entity (λ (($x Entity)) (Bind (($s Scale (Context))) (gerku $x))) (λ (($w (Referents Entity))) (CloseWith (row jmaji 1 direct-event (1)) ((1 $w))))) is not in my domain"))
+  (case (id "9950bcb96b07982d231b52cb8af364c40cb79561")
+    (status available)
+    (term
+     (Bind
+      ($w1 :: (Referents Entity))
+      (Presuppose
+       (∃ (λ (($x :: Entity)) (gerku $x)))
+       (Refer
+        (λ (($reference :: (Referents Entity)))
+          (∧
+           (∧
+            (∀ (λ (($member :: Entity)) (→ (Among $member $reference) ((λ (($x :: Entity)) (gerku $x)) $member))))
+            (∀
+             (λ (($subreference :: (Referents Entity)))
+               (→
+                (Among $subreference $reference)
+                (∃
+                 (λ (($member :: Entity))
+                   (∧
+                    ((λ (($x :: Entity)) (gerku $x)) $member)
+                    (∃
+                     (λ (($common :: (Referents Entity)))
+                       (∧ (Among $common $member) (Among $common $subreference)))))))))))
+           (∀ (λ (($member :: Entity)) (→ ((λ (($x :: Entity)) (gerku $x)) $member) (Among $member $reference))))))))
+      (∀
+       (λ (($member :: Entity))
+         (→
+          (Among $member $w1)
+          ((λ (($w :: (Referents Entity)))
+             (CloseClause
+              (λ (($actual_event :: (Referents Eventuality)))
+                (∧ ((λ (($event :: (Referents Eventuality))) (jmaji $w $event)) $actual_event) (fasnu $actual_event)))))
+           $member)))))))
+  (case (id "997aadf61f2b9a8b77acdb90390719fef358c2b5")
+    (status available)
+    (term
+     (Bind
+      ($r :: (Referents Entity))
+      (Refer (λ (($unit :: (Referents Entity))) (mlatu $unit)))
+      (Assert
+       (Bind
+        ($w1 :: (Referents Entity))
+        (SelectExactly 3 (λ (($x :: Entity)) (gerku $x)))
+        ((λ (($w :: (Referents Entity)))
+           (Bind
+            ($ctx3 :: (Referents Entity))
+            (Context)
+            (CloseClause
+             (λ (($actual_event :: (Referents Eventuality)))
+               (∧
+                ((λ (($event :: (Referents Eventuality))) (tavla $w $r $ctx3 $event)) $actual_event)
+                (fasnu $actual_event))))))
+         $w1))))))
+  (case (id "9a6d68b66792504622ef5443bf9cdab8db165f01")
+    (status available)
+    (term
+     (λ (($x :: (Referents Entity)))
+       (Bind
+        ($ctx1 :: (Referents Entity))
+        (Context)
+        ($ctx3 :: (Referents Entity))
+        (Context)
+        ($ctx4 :: (Referents Entity))
+        (Context)
+        ($ctx5 :: (Referents Entity))
+        (Context)
+        (CloseClause
+         (λ (($actual_event :: (Referents Eventuality)))
+           (∧
+            ((λ (($event :: (Referents Eventuality))) (klama $ctx1 $x $ctx3 $ctx4 $ctx5 $event)) $actual_event)
+            (fasnu $actual_event))))))))
+  (case (id "9c1407e2953b9b8ea62d6c2623bf886058927595")
+    (status available)
+    (term
+     (Bind
+      ($r :: (Referents Entity))
+      (Refer (λ (($unit :: (Referents Entity))) (gerku $unit)))
+      (Assert
+       (CloseClause
+        (λ (($actual_event :: (Referents Eventuality)))
+          (∧ ((StateClause (blabi $r)) $actual_event) (fasnu $actual_event))))))))
+  (case (id "9d479ff45f970013a08eaf988ae266bddb2e6820")
+    (status available)
+    (term
+     (Bind
+      ($r :: (Referents Entity))
+      (Refer (λ (($named :: (Referents Entity))) (Named "alis" $named)))
+      (Assert
+       (Bind
+        ($w1 :: (Referents Entity))
+        (SelectExactly 3 (λ (($x :: Entity)) (gerku $x)))
+        ((λ (($w :: (Referents Entity)))
+           (Bind
+            ($ctx3 :: (Referents Entity))
+            (Context)
+            (CloseClause
+             (λ (($actual_event :: (Referents Eventuality)))
+               (∧
+                ((λ (($event :: (Referents Eventuality))) (tavla $r $w $ctx3 $event)) $actual_event)
+                (fasnu $actual_event))))))
+         $w1))))))
+  (case (id "9e06566d9890b2c704417adef0a5b50d9cdcd8e4")
+    (status available)
+    (term
+     (Bind
+      ($nuclear_bajra_2 :: (Referents Entity))
+      (Context)
+      ($nuclear_bajra_3 :: (Referents Entity))
+      (Context)
+      ($nuclear_bajra_4 :: (Referents Entity))
+      (Context)
+      (=
+       (Card
+        (SetOf
+         (λ (($global_member :: Entity))
+           (∧
+            ((λ (($restrictor_member :: Entity)) (gerku $restrictor_member)) $global_member)
+            ((λ (($nuclear_member :: Entity))
+               (CloseClause
+                (λ (($actual_event :: (Referents Eventuality)))
+                  (∧
+                   ((λ (($event :: (Referents Eventuality)))
+                      (bajra $nuclear_member $nuclear_bajra_2 $nuclear_bajra_3 $nuclear_bajra_4 $event))
+                    $actual_event)
+                   (fasnu $actual_event)))))
+             $global_member)))))
+       3))))
+  (case (id "9e1244208e96d43b67c311bf34bbe418b2a02514")
+    (status available)
+    (term
+     (Bind
+      ($cat :: (Referents Entity))
+      (Refer (λ (($x :: (Referents Entity))) (∧ (mlatu $x) (blabi $x))))
+      (Assert
+       (Bind
+        ($ctx2 :: (Referents Entity))
+        (Context)
+        ($ctx3 :: (Referents Entity))
+        (Context)
+        (CloseClause
+         (λ (($actual_event :: (Referents Eventuality)))
+           (∧
+            ((λ (($event :: (Referents Eventuality))) (jbena $cat $ctx2 $ctx3 $event)) $actual_event)
+            (fasnu $actual_event)))))))))
+  (case (id "9eb692db840e8b2093a85c697191a3a561335644")
+    (status available)
+    (term
+     (Bind
+      ($nuclear_tavla_3 :: (Referents Entity))
+      (Context)
+      (Assert
+       (=
+        (Card
+         (SetOf
+          (λ (($global_member :: Entity))
+            (∧
+             ((λ (($restrictor_member :: Entity)) (gerku $restrictor_member)) $global_member)
+             ((λ (($nuclear_member :: Entity))
+                (CloseClause
+                 (λ (($actual_event :: (Referents Eventuality)))
+                   (∧
+                    ((λ (($event :: (Referents Eventuality))) (tavla Speaker $nuclear_member $nuclear_tavla_3 $event))
+                     $actual_event)
+                    (fasnu $actual_event)))))
+              $global_member)))))
+        3)))))
+  (case (id "a13da18fac2b9d1a13e06cf1ecc0c540d5adf01e")
+    (status unavailable)
+    (reason
+     "b1-expand-fewer-than: (b1-expand-fewer-than 1 Entity (λ (($x Entity)) (gerku $x)) (λ (($w (Referents Entity))) (Bind (($s Scale (Context))) (CloseWith (row jmaji 1 direct-event (1)) ((1 $w)))))) is not in my domain"))
+  (case (id "a276ef47aa851126f08e68dcf950821a4344f119")
+    (status unavailable)
+    (reason
+     "b1-expand-fewer-than: (b1-expand-fewer-than 1 Entity (λ (($x Entity)) (Bind (($s Scale (Context))) (gerku $x))) (λ (($w (Referents Entity))) (CloseWith (row jmaji 1 direct-event (1)) ((1 $w))))) is not in my domain"))
+  (case (id "a52f77e5f64ace85eb112472d016486a31befafa")
+    (status available)
+    (term
+     (Bind
+      ($left :: (Referents Entity))
+      (SelectExactly 3 (λ (($x :: Entity)) (gerku $x)))
+      ($right :: (Referents Entity))
+      (SelectExactly 2 (λ (($x1 :: Entity)) (prenu $x1)))
+      (Mention
+       (∀
+        (λ (($member :: Entity))
+          (→
+           (Among $member $left)
+           ((λ (($l :: Entity))
+              (∀
+               (λ (($member :: Entity))
+                 (→
+                  (Among $member $right)
+                  ((λ (($r :: Entity))
+                     (CloseClause
+                      (λ (($actual_event :: (Referents Eventuality)))
+                        (∧ ((StateClause (nelci $l $r)) $actual_event) (fasnu $actual_event)))))
+                   $member)))))
+            $member))))))))
+  (case (id "a6c8d36f67dc1c2896c84ec3fa881889f761b7d4")
+    (status available)
+    (term
+     (Assert
+      (¬
+       (Bind
+        ($w1 :: (Referents Entity))
+        (SelectAtLeast 1 (λ (($x :: Entity)) (gerku $x)))
+        ((λ (($w :: (Referents Entity)))
+           (Bind
+            ($ctx3 :: (Referents Entity))
+            (Context)
+            (CloseClause
+             (λ (($actual_event :: (Referents Eventuality)))
+               (∧
+                ((λ (($event :: (Referents Eventuality))) (tavla Speaker $w $ctx3 $event)) $actual_event)
+                (fasnu $actual_event))))))
+         $w1))))))
+  (case (id "a80380a1b22f80fe8a622376789319b054091307")
+    (status available)
+    (term
+     (Mention
+      (Bind
+       ($w1 :: (Referents Entity))
+       (SelectAtLeast 1 (λ (($x :: Entity)) (gerku $x)))
+       ((λ (($w :: (Referents Entity)))
+          (Bind
+           ($ctx3 :: (Referents Entity))
+           (Context)
+           (CloseClause
+            (λ (($actual_event :: (Referents Eventuality)))
+              (∧
+               ((λ (($event :: (Referents Eventuality))) (tavla $w Speaker $ctx3 $event)) $actual_event)
+               (fasnu $actual_event))))))
+        $w1)))))
+  (case (id "adaf5b13f560e52ca23d027a2d22093fa35294bb")
+    (status unavailable)
+    (reason
+     "b1-expand-at-least: no clauses matched for (b1-expand-at-least $n Entity (λ (($x Entity)) (mlatu $x)) (λ (($w (Referents Entity))) (CloseWith (row tavla 3 direct-event (1 2 3)) ((1 $r) (2 $w)))))"))
+  (case (id "ae0905b127f17eec2dd17799de3b6e64a28f0423")
+    (status available)
+    (term
+     (Bind
+      ($purpose :: (Referents Entity))
+      (Context)
+      ($n :: Natural)
+      (Vague (AdmissibleThreshold TooManyK (λ (($x :: Entity)) (gerku $x)) $purpose))
+      (Assert
+       (Bind
+        ($w1 :: (Referents Entity))
+        (SelectAtLeast (+ $n 1) (λ (($x :: Entity)) (gerku $x)))
+        ((λ (($w :: (Referents Entity)))
+           (Bind
+            ($ctx2 :: (Referents Entity))
+            (Context)
+            ($ctx3 :: (Referents Entity))
+            (Context)
+            ($ctx4 :: (Referents Entity))
+            (Context)
+            ($ctx5 :: (Referents Entity))
+            (Context)
+            (CloseClause
+             (λ (($actual_event :: (Referents Eventuality)))
+               (∧
+                ((λ (($event :: (Referents Eventuality))) (klama $w $ctx2 $ctx3 $ctx4 $ctx5 $event)) $actual_event)
+                (fasnu $actual_event))))))
+         $w1))))))
+  (case (id "afdc655e5d92abe64d7f60264ba07d4e6d7aac18")
+    (status available)
+    (term
+     (Bind
+      ($nuclear_bajra_2 :: (Referents Entity))
+      (Context)
+      ($nuclear_bajra_3 :: (Referents Entity))
+      (Context)
+      ($nuclear_bajra_4 :: (Referents Entity))
+      (Context)
+      (Mention
+       (=
+        (Card
+         (SetOf
+          (λ (($global_member :: Entity))
+            (∧
+             ((λ (($restrictor_member :: Entity)) (gerku $restrictor_member)) $global_member)
+             ((λ (($nuclear_member :: Entity))
+                (CloseClause
+                 (λ (($actual_event :: (Referents Eventuality)))
+                   (∧
+                    ((λ (($event :: (Referents Eventuality)))
+                       (bajra $nuclear_member $nuclear_bajra_2 $nuclear_bajra_3 $nuclear_bajra_4 $event))
+                     $actual_event)
+                    (fasnu $actual_event)))))
+              $global_member)))))
+        3)))))
+  (case (id "b03bdb8567704858bc0414f946cd16154278b6ca")
+    (status available)
+    (term
+     (Mention
+      (λ (($x :: (Referents Entity)))
+        (Bind
+         ($ctx1 :: (Referents Entity))
+         (Context)
+         ($ctx3 :: (Referents Entity))
+         (Context)
+         ($ctx4 :: (Referents Entity))
+         (Context)
+         ($ctx5 :: (Referents Entity))
+         (Context)
+         (CloseClause
+          (λ (($actual_event :: (Referents Eventuality)))
+            (∧
+             ((λ (($event :: (Referents Eventuality))) (klama $ctx1 $x $ctx3 $ctx4 $ctx5 $event)) $actual_event)
+             (fasnu $actual_event)))))))))
+  (case (id "b4f5a39f1b309245b2d50930cb69faed4a7b4716")
+    (status available)
+    (term
+     (Bind
+      ($a :: (Referents Amount))
+      (Refer
+       (λ (($x :: (Referents Amount)))
+         (Close
+          ((NiRel
+            (Bind
+             ($ctx2 :: (Referents Entity))
+             (Context)
+             ($ctx3 :: (Referents Entity))
+             (Context)
+             ($ctx4 :: (Referents Entity))
+             (Context)
+             ($ctx5 :: (Referents Entity))
+             (Context)
+             (CloseClause
+              (λ (($actual_event :: (Referents Eventuality)))
+                (∧
+                 ((λ (($event :: (Referents Eventuality))) (klama Speaker $ctx2 $ctx3 $ctx4 $ctx5 $event))
+                  $actual_event)
+                 (fasnu $actual_event))))))
+           $x))))
+      (Mention $a))))
+  (case (id "b92059ed2600b14c09f0cbb9515567e36d32a11b")
+    (status available)
+    (term
+     (Assert
+      (¬
+       (Bind
+        ($w1 :: (Referents Entity))
+        (SelectAtLeast 1 (λ (($x :: Entity)) (gerku $x)))
+        ((λ (($w :: (Referents Entity)))
+           (Bind
+            ($ctx3 :: (Referents Entity))
+            (Context)
+            (CloseClause
+             (λ (($actual_event :: (Referents Eventuality)))
+               (∧
+                ((λ (($event :: (Referents Eventuality))) (tavla $w Speaker $ctx3 $event)) $actual_event)
+                (fasnu $actual_event))))))
+         $w1))))))
+  (case (id "b96bfb9de1d104d2377dbf04658ed8c492dcde96")
+    (status available)
+    (term
+     (Bind
+      ($r :: (Referents Entity))
+      (Refer (λ (($unit1 :: (Referents Entity))) (gerku $unit1)))
+      (Bind
+       ($r1 :: (Referents Entity))
+       (Refer (λ (($unit :: (Referents Entity))) (mlatu $unit)))
+       (Assert
+        (Bind
+         ($ctx3 :: (Referents Entity))
+         (Context)
+         (CloseClause
+          (λ (($actual_event :: (Referents Eventuality)))
+            (∧
+             ((λ (($event :: (Referents Eventuality))) (tavla $r $r1 $ctx3 $event)) $actual_event)
+             (fasnu $actual_event))))))))))
+  (case (id "bb1ea3fc5780f5d106de8232523d33221406da46")
+    (status available)
+    (term
+     (Bind
+      ($r :: (Referents Entity))
+      (Refer (λ (($unit :: (Referents Entity))) (mlatu $unit)))
+      (Assert
+       (Bind
+        ($w1 :: (Referents Entity))
+        (SelectAtLeast 1 (λ (($x :: Entity)) (gerku $x)))
+        ((λ (($w :: (Referents Entity)))
+           (Bind
+            ($ctx3 :: (Referents Entity))
+            (Context)
+            (CloseClause
+             (λ (($actual_event :: (Referents Eventuality)))
+               (∧
+                ((λ (($event :: (Referents Eventuality))) (tavla $w $r $ctx3 $event)) $actual_event)
+                (fasnu $actual_event))))))
+         $w1))))))
+  (case (id "bd272fdf0064b6f7f1a30d72aaa6909228be68f7")
+    (status available)
+    (term
+     (Bind
+      ($bob :: (Referents Entity))
+      (Refer (λ (($x :: (Referents Entity))) (Named "bab" $x)))
+      (Do
+       (Assert
+        (Bind
+         ($ctx2 :: (Referents Entity))
+         (Context)
+         ($ctx3 :: (Referents Entity))
+         (Context)
+         ($ctx4 :: (Referents Entity))
+         (Context)
+         ($ctx5 :: (Referents Entity))
+         (Context)
+         (CloseClause
+          (λ (($actual_event :: (Referents Eventuality)))
+            (∧
+             ((λ (($event :: (Referents Eventuality))) (klama $bob $ctx2 $ctx3 $ctx4 $ctx5 $event)) $actual_event)
+             (fasnu $actual_event))))))
+       (Assert
+        (Bind
+         ($ctx2 :: (Referents Entity))
+         (Context)
+         (CloseClause
+          (λ (($actual_event :: (Referents Eventuality)))
+            (∧ ((StateClause (prami $bob $ctx2)) $actual_event) (fasnu $actual_event))))))))))
+  (case (id "c09304c3c5c8c1202284e2acc37d191b7a50bb11")
+    (status available)
+    (term
+     (Bind
+      ($r :: (Referents Entity))
+      (Refer (λ (($unit :: (Referents Entity))) (mlatu $unit)))
+      (Bind
+       ($nuclear_tavla_3 :: (Referents Entity))
+       (Context)
+       (Assert
+        (=
+         (Card
+          (SetOf
+           (λ (($global_member :: Entity))
+             (∧
+              ((λ (($restrictor_member :: Entity)) (gerku $restrictor_member)) $global_member)
+              ((λ (($nuclear_member :: Entity))
+                 (CloseClause
+                  (λ (($actual_event :: (Referents Eventuality)))
+                    (∧
+                     ((λ (($event :: (Referents Eventuality))) (tavla $r $nuclear_member $nuclear_tavla_3 $event))
+                      $actual_event)
+                     (fasnu $actual_event)))))
+               $global_member)))))
+         3))))))
+  (case (id "c27acb49649a24ec94cecaf88567f2d8e9165026")
+    (status available)
+    (term
+     (Bind
+      ($w :: (Referents Entity))
+      (SelectExactly 3 (λ (($x :: Entity)) (gerku $x)))
+      (Bind
+       ($ctx2 :: (Referents Entity))
+       (Context)
+       ($ctx3 :: (Referents Entity))
+       (Context)
+       ($ctx4 :: (Referents Entity))
+       (Context)
+       (CloseClause
+        (λ (($actual_event :: (Referents Eventuality)))
+          (∧
+           ((λ (($event :: (Referents Eventuality))) (bajra $w $ctx2 $ctx3 $ctx4 $event)) $actual_event)
+           (fasnu $actual_event))))))))
+  (case (id "c2893c48f65e9358154c3c71c07d9f10e125e8b4")
+    (status available)
+    (term
+     (Assert
+      (Bind
+       ($w2 :: (Referents Entity))
+       (SelectExactly 3 (λ (($x :: Entity)) (gerku $x)))
+       ((λ (($w :: (Referents Entity)))
+          (Bind
+           ($w2 :: (Referents Entity))
+           (SelectExactly 2 (λ (($x :: Entity)) (mlatu $x)))
+           ((λ (($w1 :: (Referents Entity)))
+              (Bind
+               ($ctx3 :: (Referents Entity))
+               (Context)
+               (CloseClause
+                (λ (($actual_event :: (Referents Eventuality)))
+                  (∧
+                   ((λ (($event :: (Referents Eventuality))) (tavla $w $w1 $ctx3 $event)) $actual_event)
+                   (fasnu $actual_event))))))
+            $w2)))
+        $w2)))))
+  (case (id "c3ef43fc929c9a2356838ee5d5de4bea0a7d5b0d")
+    (status available)
+    (term (λ (($p :: (PredTerm (RowOf zzzz)))) (Close $p))))
+  (case (id "c3f807759c2a4b21cc592b0ff7b4858dbd44f1a8")
+    (status unavailable)
+    (reason
+     "a0-expand-let: (a0-expand-let $prior (Act Assertion) (Assert (CloseWith (row klama 5 direct-event (1 2 3 4 5)) ((1 Audience)))) (Bind (($prioro (ActOccurrence Assertion) (Perform Host $prior))) (Bind (($defect DefectKind (Context))) (Express (Close (MetalinguisticallyDefective $prioro $defect)))))) is not in my domain"))
+  (case (id "c5058c35cd20c0e848804a9b2e0fa31c745e3885")
+    (status available)
+    (term
+     (λ (($p :: (Fn (Entity) Content)) ($r :: (Referents Entity)))
+       (∧
+        (∀ (λ (($member :: Entity)) (→ (Among $member $r) ($p $member))))
+        (∀
+         (λ (($subreference :: (Referents Entity)))
+           (→
+            (Among $subreference $r)
+            (∃
+             (λ (($member :: Entity))
+               (∧
+                ($p $member)
+                (∃
+                 (λ (($common :: (Referents Entity)))
+                   (∧ (Among $common $member) (Among $common $subreference))))))))))))))
+  (case (id "c514182c124a29774fb65f68a9f1b73a31b5130b")
+    (status available)
+    (term
+     (λ (($k :: (DecompositionBasis (Group Entity) Entity)))
+       (Bind
+        ($g :: (Referents (Group Entity)))
+        (SelectExactly
+         1
+         (λ (($group :: (Group Entity)))
+           (∧
+            (Aggregate $k $group)
+            (∧
+             (∀
+              (λ (($basis_unit :: (Referents Entity)))
+                (→
+                 (BasisUnitAt $k $basis_unit Speaker)
+                 (∃
+                  (λ (($peer_unit :: (Referents Entity)))
+                    (∧
+                     (PeerUnitAt $k $peer_unit $group)
+                     (∧ (Among $basis_unit $peer_unit) (Among $peer_unit $basis_unit))))))))
+             (∀
+              (λ (($complete_peer :: (Referents Entity)))
+                (→
+                 (PeerUnitAt $k $complete_peer $group)
+                 (∃
+                  (λ (($complete_unit :: (Referents Entity)))
+                    (∧
+                     (BasisUnitAt $k $complete_unit Speaker)
+                     (∧ (Among $complete_unit $complete_peer) (Among $complete_peer $complete_unit))))))))))))
+        (Mention $g)))))
+  (case (id "cb0c2d14a541bd5721c594d8492a196ae21fc449")
+    (status available)
+    (term
+     ((λ (($a :: (Act Assertion))) (Do (Perform $a) (Perform $a)))
+      (Assert
+       (Bind
+        ($ctx2 :: (Referents Entity))
+        (Context)
+        ($ctx3 :: (Referents Entity))
+        (Context)
+        ($ctx4 :: (Referents Entity))
+        (Context)
+        ($ctx5 :: (Referents Entity))
+        (Context)
+        (CloseClause
+         (λ (($actual_event :: (Referents Eventuality)))
+           (∧
+            ((λ (($event :: (Referents Eventuality))) (klama Speaker $ctx2 $ctx3 $ctx4 $ctx5 $event)) $actual_event)
+            (fasnu $actual_event)))))))))
+  (case (id "cb238239f922d167cfddd4bbb3dfeaea323ce103")
+    (status unavailable)
+    (reason "m2-oracle: Massify basis type unavailable"))
+  (case (id "cb8093665b4b7ed893a755ddf7595d703673c951")
+    (status available)
+    (term
+     (SetOf
+      (λ (($z :: Entity))
+        (Bind
+         ($w1 :: (Referents Entity))
+         (SelectAtLeast 1 (λ (($x :: Entity)) (gerku $x)))
+         ((λ (($w :: (Referents Entity)))
+            (CloseClause
+             (λ (($actual_event :: (Referents Eventuality)))
+               (∧ ((λ (($event :: (Referents Eventuality))) (jmaji $w $event)) $actual_event) (fasnu $actual_event)))))
+          $w1))))))
+  (case (id "cf2374e6e207721068753ffa99278a37b7d56886")
+    (status available)
+    (term
+     (Assert
+      (Bind
+       ($w :: (Referents Entity))
+       (Presuppose
+        (∃ (λ (($x :: Entity)) (gerku $x)))
+        (Refer
+         (λ (($reference :: (Referents Entity)))
+           (∧
+            (∧
+             (∀ (λ (($member :: Entity)) (→ (Among $member $reference) ((λ (($x :: Entity)) (gerku $x)) $member))))
+             (∀
+              (λ (($subreference :: (Referents Entity)))
+                (→
+                 (Among $subreference $reference)
+                 (∃
+                  (λ (($member :: Entity))
+                    (∧
+                     ((λ (($x :: Entity)) (gerku $x)) $member)
+                     (∃
+                      (λ (($common :: (Referents Entity)))
+                        (∧ (Among $common $member) (Among $common $subreference)))))))))))
+            (∀ (λ (($member :: Entity)) (→ ((λ (($x :: Entity)) (gerku $x)) $member) (Among $member $reference))))))))
+       (∀
+        (λ (($member :: Entity))
+          (→
+           (Among $member $w)
+           ((λ (($x :: Entity))
+              (Bind
+               ($ctx3 :: (Referents Entity))
+               (Context)
+               (CloseClause
+                (λ (($actual_event :: (Referents Eventuality)))
+                  (∧
+                   ((λ (($event :: (Referents Eventuality))) (tavla Speaker $x $ctx3 $event)) $actual_event)
+                   (fasnu $actual_event))))))
+            $member))))))))
+  (case (id "d12cc9e49c7b44ac7c5244121e90ff57baa5d4a7")
+    (status unavailable)
+    (reason
+     "b1-expand-at-most: (b1-expand-at-most 1 Entity (λ (($x Entity)) (Bind (($s Scale (Context))) (gerku $x))) (λ (($w (Referents Entity))) (CloseWith (row jmaji 1 direct-event (1)) ((1 $w))))) is not in my domain"))
+  (case (id "d6acabd21a4c2aef89fc166afdabe8cb838beaa1")
+    (status available)
+    (term
+     (Bind
+      ($r :: (Referents Entity))
+      (Refer (λ (($unit :: (Referents Entity))) (mlatu $unit)))
+      (Assert
+       (¬
+        (Bind
+         ($w1 :: (Referents Entity))
+         (SelectAtLeast 1 (λ (($x :: Entity)) (gerku $x)))
+         ((λ (($w :: (Referents Entity)))
+            (Bind
+             ($ctx3 :: (Referents Entity))
+             (Context)
+             (CloseClause
+              (λ (($actual_event :: (Referents Eventuality)))
+                (∧
+                 ((λ (($event :: (Referents Eventuality))) (tavla $w $r $ctx3 $event)) $actual_event)
+                 (fasnu $actual_event))))))
+          $w1)))))))
+  (case (id "d7c04355b8abb979b3e68ab4cb224f4617b83534")
+    (status available)
+    (term
+     (Bind
+      ($r :: (Referents Entity))
+      (Refer (λ (($unit :: (Referents Entity))) (mlatu $unit)))
+      (Assert
+       (Bind
+        ($w1 :: (Referents Entity))
+        (SelectAtLeast 1 (λ (($x :: Entity)) (gerku $x)))
+        ((λ (($w :: (Referents Entity)))
+           (Bind
+            ($ctx3 :: (Referents Entity))
+            (Context)
+            (CloseClause
+             (λ (($actual_event :: (Referents Eventuality)))
+               (∧
+                ((λ (($event :: (Referents Eventuality))) (tavla $r $w $ctx3 $event)) $actual_event)
+                (fasnu $actual_event))))))
+         $w1))))))
+  (case (id "d8e9f58244e983851351b588de235d4375f926f0")
+    (status available)
+    (term
+     (λ (($p :: (Fn (Eventuality) Content)) ($r :: (Referents Entity)))
+       (∧
+        (∀ (λ (($member :: Entity)) (→ (Among $member $r) ($p $member))))
+        (∀
+         (λ (($subreference :: (Referents Eventuality)))
+           (→
+            (Among $subreference $r)
+            (∃
+             (λ (($member :: Eventuality))
+               (∧
+                ($p $member)
+                (∃
+                 (λ (($common :: (Referents Eventuality)))
+                   (∧ (Among $common $member) (Among $common $subreference))))))))))))))
+  (case (id "d9e452a092108b6bfaec9670967ce2aa285e61d4")
+    (status available)
+    (term
+     (Ask
+      (OpenQ
+       (λ (($x :: (Referents Entity)))
+         (Bind
+          ($ctx2 :: (Referents Entity))
+          (Context)
+          ($ctx3 :: (Referents Entity))
+          (Context)
+          ($ctx4 :: (Referents Entity))
+          (Context)
+          ($ctx5 :: (Referents Entity))
+          (Context)
+          (CloseClause
+           (λ (($actual_event :: (Referents Eventuality)))
+             (∧
+              ((λ (($event :: (Referents Eventuality))) (klama $x $ctx2 $ctx3 $ctx4 $ctx5 $event)) $actual_event)
+              (fasnu $actual_event))))))))))
+  (case (id "da97e598f0594e6ba811953858f978a3c3a9528f")
+    (status available)
+    (term
+     (Assert
+      (¬
+       (Bind
+        ($w1 :: (Referents Entity))
+        (SelectAtLeast 1 (λ (($x :: Entity)) (prenu $x)))
+        ((λ (($w :: (Referents Entity)))
+           (CloseClause
+            (λ (($actual_event :: (Referents Eventuality)))
+              (∧ ((λ (($event :: (Referents Eventuality))) (jmaji $w $event)) $actual_event) (fasnu $actual_event)))))
+         $w1))))))
+  (case (id "db9e84ebb83dc304f85923c2946dc35e1a13993e")
+    (status available)
+    (term
+     (Bind
+      ($nuclear_bajra_2 :: (Referents Entity))
+      (Context)
+      ($nuclear_bajra_3 :: (Referents Entity))
+      (Context $nuclear_bajra_2)
+      ($nuclear_bajra_4 :: (Referents Entity))
+      (Context)
+      (=
+       (Card
+        (SetOf
+         (λ (($global_member :: Entity))
+           (∧
+            ((λ (($restrictor_member :: Entity)) (gerku $restrictor_member)) $global_member)
+            ((λ (($nuclear_member :: Entity))
+               (CloseClause
+                (λ (($actual_event :: (Referents Eventuality)))
+                  (∧
+                   ((λ (($event :: (Referents Eventuality)))
+                      (bajra $nuclear_member $nuclear_bajra_2 $nuclear_bajra_3 $nuclear_bajra_4 $event))
+                    $actual_event)
+                   (fasnu $actual_event)))))
+             $global_member)))))
+       3))))
+  (case (id "dd044fa4f64eeccef4d68d8a20fccc9210219397")
+    (status available)
+    (term
+     (Bind
+      ($cat :: (Referents Entity))
+      (Refer (λ (($x :: (Referents Entity))) (mlatu $x)))
+      (Assert
+       (CloseClause
+        (λ (($actual_event :: (Referents Eventuality)))
+          (∧ ((StateClause (blabi $cat)) $actual_event) (fasnu $actual_event))))))))
+  (case (id "e23de12dfd8d47e7979803ed3f6c7f0f7b6517fa")
+    (status available)
+    (term
+     (Generic
+      Typical
+      (λ (($x :: Entity)) (Bind ($s :: Scale) (Context) (gerku $x)))
+      (λ (($x :: Entity))
+        (CloseClause
+         (λ (($actual_event :: (Referents Eventuality)))
+           (∧ ((λ (($event :: (Referents Eventuality))) (jmaji $x $event)) $actual_event) (fasnu $actual_event))))))))
+  (case (id "e265f654d73091e8db042b5820cba0df47e812be")
+    (status unavailable)
+    (reason
+     "a0-expand-let: (a0-expand-let $a (Act Assertion) (Assert (CloseWith (row cadzu 4 direct-event (1 2 3 4)) ((1 Audience)))) (Bind (($o (ActOccurrence Assertion) (Perform Host $a))) (Do (Perform AttachedDisplay (Express (Close (EvidentialBasis Speaker $o Observation))))))) is not in my domain"))
+  (case (id "e4a28c0b1783335f69507f29ca64cc782b80c7be")
+    (status available)
+    (term
+     (Bind
+      ($dogs :: (Referents Entity))
+      (SelectExactly 3 (λ (($x :: Entity)) (gerku $x)))
+      (Do
+       (Assert
+        (Bind
+         ($ctx2 :: (Referents Entity))
+         (Context)
+         ($ctx3 :: (Referents Entity))
+         (Context)
+         ($ctx4 :: (Referents Entity))
+         (Context)
+         (CloseClause
+          (λ (($actual_event :: (Referents Eventuality)))
+            (∧
+             ((λ (($event :: (Referents Eventuality))) (bajra $dogs $ctx2 $ctx3 $ctx4 $event)) $actual_event)
+             (fasnu $actual_event))))))
+       (Assert
+        (CloseClause
+         (λ (($actual_event :: (Referents Eventuality)))
+           (∧ ((StateClause (tatpi $dogs)) $actual_event) (fasnu $actual_event)))))))))
+  (case (id "e666727fbb4c77fa54491719b49600cb4db7303a")
+    (status available)
+    (term
+     (Bind
+      ($r :: (Referents Entity))
+      (Refer (λ (($named :: (Referents Entity))) (Named "alis" $named)))
+      (Assert
+       (Bind
+        ($ctx2 :: (Referents Entity))
+        (Context)
+        ($ctx3 :: (Referents Entity))
+        (Context)
+        ($ctx4 :: (Referents Entity))
+        (Context)
+        ($ctx5 :: (Referents Entity))
+        (Context)
+        (CloseClause
+         (λ (($actual_event :: (Referents Eventuality)))
+           (∧
+            ((λ (($event :: (Referents Eventuality))) (klama $r $ctx2 $ctx3 $ctx4 $ctx5 $event)) $actual_event)
+            (fasnu $actual_event)))))))))
+  (case (id "e69b9851e31ac7dae947e10cb7bd7ddeedeca790")
+    (status available)
+    (term
+     (Bind
+      ($r :: (Referents Entity))
+      (Refer (λ (($unit :: (Referents Entity))) (mlatu $unit)))
+      (Assert
+       (Bind
+        ($w :: (Referents Entity))
+        (Presuppose
+         (∃ (λ (($x :: Entity)) (gerku $x)))
+         (Refer
+          (λ (($reference :: (Referents Entity)))
+            (∧
+             (∧
+              (∀ (λ (($member :: Entity)) (→ (Among $member $reference) ((λ (($x :: Entity)) (gerku $x)) $member))))
+              (∀
+               (λ (($subreference :: (Referents Entity)))
+                 (→
+                  (Among $subreference $reference)
+                  (∃
+                   (λ (($member :: Entity))
+                     (∧
+                      ((λ (($x :: Entity)) (gerku $x)) $member)
+                      (∃
+                       (λ (($common :: (Referents Entity)))
+                         (∧ (Among $common $member) (Among $common $subreference)))))))))))
+             (∀ (λ (($member :: Entity)) (→ ((λ (($x :: Entity)) (gerku $x)) $member) (Among $member $reference))))))))
+        (∀
+         (λ (($member :: Entity))
+           (→
+            (Among $member $w)
+            ((λ (($x :: Entity))
+               (Bind
+                ($ctx3 :: (Referents Entity))
+                (Context)
+                (CloseClause
+                 (λ (($actual_event :: (Referents Eventuality)))
+                   (∧
+                    ((λ (($event :: (Referents Eventuality))) (tavla $r $x $ctx3 $event)) $actual_event)
+                    (fasnu $actual_event))))))
+             $member)))))))))
+  (case (id "e6de3a77f1ef095f2c747f051f659f74f57ebab3")
+    (status available)
+    (term
+     (Bind
+      ($o :: (ActOccurrence Assertion))
+      (Local
+       (Perform
+        (Assert
+         (CloseClause
+          (λ (($actual_event :: (Referents Eventuality)))
+            (∧ ((StateClause (gerku Speaker)) $actual_event) (fasnu $actual_event)))))))
+      (Mention $o))))
+  (case (id "e72922e2754b6fbae2733c861813fd899a07eb3a")
+    (status available)
+    (term
+     (Express
+      (Close
+       (Desire
+        Speaker
+        (Reify
+         (CloseClause
+          (λ (($actual_event :: (Referents Eventuality)))
+            (∧
+             ((λ (($event :: (Referents Eventuality))) (sipna Speaker $event)) $actual_event)
+             (fasnu $actual_event))))))))))
+  (case (id "e97a3f27befc567d541ac57e93d47c88db3e5370")
+    (status available)
+    (term ((λ (($a :: (Act Assertion))) (Mention $a)) (Mention Speaker))))
+  (case (id "ec2d5fbe1f794cd8f00cd46255188ca070b7f0c1")
+    (status available)
+    (term
+     (Bind
+      ($surface :: (Referents Entity))
+      (Context)
+      ($limbs :: (Referents Entity))
+      (Context)
+      ($gait :: (Referents Entity))
+      (Context)
+      (=
+       (Card
+        (SetOf
+         (λ (($x :: Entity))
+           (∧
+            (gerku $x)
+            (CloseClause
+             (λ (($actual_event :: (Referents Eventuality)))
+               (∧
+                ((λ (($event :: (Referents Eventuality))) (bajra $x $surface $limbs $gait $event)) $actual_event)
+                (fasnu $actual_event))))))))
+       3))))
+  (case (id "ef0d085f9a8c3af028bb48b3c99f40d636cb9385")
+    (status available)
+    (term
+     (Bind
+      ($r :: (Referents Entity))
+      (Refer (λ (($named :: (Referents Entity))) (Named "alis" $named)))
+      (Assert
+       (Bind
+        ($ctx3 :: (Referents Entity))
+        (Context)
+        (CloseClause
+         (λ (($actual_event :: (Referents Eventuality)))
+           (∧
+            ((λ (($event :: (Referents Eventuality))) (tavla $r Speaker $ctx3 $event)) $actual_event)
+            (fasnu $actual_event)))))))))
+  (case (id "f653cb0a56774dea1f78c007c770b90d51c88371")
+    (status available)
+    (term
+     ((λ (($a :: (Act Assertion))) (Do (Perform $a) (Perform $a)))
+      (Assert
+       (CloseClause
+        (λ (($actual_event :: (Referents Eventuality)))
+          (∧ ((StateClause (gerku Speaker)) $actual_event) (fasnu $actual_event))))))))
+  (case (id "f695d47c0ad2f542eae100e0b6815df434e79933")
+    (status available)
+    (term
+     (Assert
+      (Presuppose
+       (∃
+        (λ (($x :: Entity))
+          (∧
+           (prenu $x)
+           (∃
+            (λ (($y :: Entity))
+              (∧
+               (xasli $y)
+               (CloseClause
+                (λ (($actual_event :: (Referents Eventuality)))
+                  (∧ ((StateClause (ponse $x $y)) $actual_event) (fasnu $actual_event))))))))))
+       (∀
+        (λ (($p :: Entity) ($d :: (Referents Entity)))
+          (→
+           (∧
+            (prenu $p)
+            (∀ (λ (($member :: Entity)) (→ (Among $member $d) ((λ (($z :: Entity)) (xasli $z)) $member))))
+            (CloseClause
+             (λ (($actual_event :: (Referents Eventuality)))
+               (∧ ((StateClause (ponse $p $d)) $actual_event) (fasnu $actual_event)))))
+           (Bind
+            ($ctx3 :: (Referents Entity))
+            (Context)
+            (CloseClause
+             (λ (($actual_event :: (Referents Eventuality)))
+               (∧
+                ((λ (($event :: (Referents Eventuality))) (darxi $p $d $ctx3 $event)) $actual_event)
+                (fasnu $actual_event))))))))))))
+  (case (id "f9f7acbbeb94b894a71e501a3ec02e82877fd496")
+    (status available)
+    (term
+     (Assert
+      (Bind
+       ($w1 :: (Referents Entity))
+       (SelectAtLeast 1 (λ (($x :: Entity)) (gerku $x)))
+       ((λ (($w :: (Referents Entity)))
+          (Bind
+           ($ctx3 :: (Referents Entity))
+           (Context)
+           (CloseClause
+            (λ (($actual_event :: (Referents Eventuality)))
+              (∧
+               ((λ (($event :: (Referents Eventuality))) (tavla Speaker $w $ctx3 $event)) $actual_event)
+               (fasnu $actual_event))))))
+        $w1)))))
+  (case (id "fb5015ae6fdfa682c9b7f70814a49daf00df1d91")
+    (status available)
+    (term
+     (SetOf
+      (λ (($z :: Entity))
+        (Bind
+         ($w1 :: (Referents Entity))
+         (SelectExactly 1 (λ (($x :: Entity)) (gerku $x)))
+         ((λ (($w :: (Referents Entity)))
+            (CloseClause
+             (λ (($actual_event :: (Referents Eventuality)))
+               (∧ ((λ (($event :: (Referents Eventuality))) (jmaji $w $event)) $actual_event) (fasnu $actual_event)))))
+          $w1))))))
+  (case (id "fdcc4eabea6f2fa114a1eef0cb43fcc0aa653e60")
+    (status unavailable)
+    (reason
+     "a0-expand-close: (a0-expand-close (row jinvi 4 holding-state (1 2 3 4)) ((1 Speaker) (2 (Reify (Let ($p Proposition) (Reify (CloseWith (row klama 5 direct-event (1 2 3 4 5)) ((1 Audience)))) (Supplement $p (Close (EvidentialBasis Speaker $p Hearsay)) (Holds $p))))))) is not in my domain"))
+  (case (id "fe81c08b40808760d2268088eb37bd2e0a092ad2")
+    (status unavailable)
+    (reason
+     "b1-expand-at-least: (b1-expand-at-least 0 Entity (λ (($x Entity)) (gerku $x)) (λ (($w (Referents Entity))) (Bind (($s Scale (Context))) (CloseWith (row jmaji 1 direct-event (1)) ((1 $w)))))) is not in my domain"))
+  (case (id "ff0589096c5b179be217803445eae85e2e574fdc")
+    (status unavailable)
+    (reason
+     "a0-expand-exactly: (a0-expand-exactly 1 Entity (λ (($x Entity)) (Bind (($s Scale (Context))) (gerku $x))) (λ (($w (Referents Entity))) (CloseWith (row jmaji 1 direct-event (1)) ((1 $w))))) is not in my domain"))))
